verify/LongLoopv3.v
@@ -1,0 +1,1129 @@
+From BusyCoq Require Import LongLoop.
+From BusyCoq Require Import Individual62.
+From BusyCoq Require LongAcc.
+
+Module LongLoop62 := LongLoop BB62.
+Import LongLoop62.
+
+Require Import ZArith.
+Require Import String.
+
+Close Scope N.
+
+Import Eqb.
+
+Ltac esx :=
+  (apply BoundedConfig.segRLs_c_spec with (T:=10^3); reflexivity) ||
+  (apply BoundedConfig.segRLs_c_spec with (T:=10^6); reflexivity) ||
+  (apply BoundedConfig.sideRLs_c_spec with (T:=10^3); reflexivity) ||
+  (eapply sideRLs_c_spec with (T:=10^6); [vm_compute; reflexivity | st; reflexivity]) ||
+  (eapply evstep_c_spec;
+   eapply Individual62.Enumerate.Permute.Flip.Compute.TM.evstep_c_spec;
+   change c0 with (Individual62.Enumerate.Permute.Flip.Compute.TM.c0);
+   cbn; solve_init).
+
+Module LongAcc62 := LongAcc.LongAcc BB62.
+
+Lemma find_spec {X Y} {E:Eqb X} (x0:X) ls (y0:Y):
+  List.find (fun '(x,y) => eqb x x0) ls &&& (fun '(x,y) => Some y) = Some y0 ->
+  List.In (x0,y0) ls.
+Proof.
+  intros.
+  unfold if_Some in H.
+  destruct (List.find (fun '(x,_) => eqb x x0)) eqn:E0.
+  2: inverts H.
+  eapply List.find_some in E0.
+  destruct E0 as [I1 I2].
+  destruct p as [x y].
+  destruct (eqb_spec x x0); [|inverts I2].
+  subst.
+  inverts H; trivial.
+Qed.
+
+Lemma f2_spec' tm ls T:
+  List.forallb (fun '(h,w,(a0,a1,h')) =>
+  BoundedConfig.segRLs_c tm ([h] ^^ N.to_nat (2 ^ a0)) ([h'] ^^ N.to_nat (2 ^ a1)) w w T) ls = true ->
+  forall w h a0 a1 h',
+  List.In (h, w, (a0, a1, h')) ls ->
+  segRLs tm ([h] ^^ N.to_nat (2 ^ a0)) ([h'] ^^ N.to_nat (2 ^ a1)) w w.
+Proof.
+  intros.
+  rewrite List.forallb_forall in H.
+  apply H in H0.
+  apply BoundedConfig.segRLs_c_spec in H0.
+  apply H0.
+Qed.
+
+Lemma f1_spec' tm ls T:
+  List.forallb (fun '(h,w,(ws,hs)) => BoundedConfig.segRLs_c tm [h] hs w (List.concat ws) T) ls = true ->
+  forall w h ws hs,
+  List.In (h, w, (ws, hs)) ls ->
+  segRLs tm [h] hs w (List.concat ws).
+Proof.
+  intros.
+  rewrite List.forallb_forall in H.
+  apply H in H0.
+  apply BoundedConfig.segRLs_c_spec in H0.
+  apply H0.
+Qed.
+
+Lemma f0_spec' tm ls T:
+  List.forallb (fun '(h,w,(ws',w')) => BoundedConfig.sideRLs_c tm [h] w ((List.concat ws')++w') T) ls = true ->
+  forall w h w',
+  List.In (h, w, w') ls ->
+  sideRLs tm [h] (w *> 0inf) (to_side w').
+Proof.
+  intros.
+  rewrite List.forallb_forall in H.
+  apply H in H0.
+  destruct w' as [ws' w'].
+  apply BoundedConfig.sideRLs_c_spec in H0.
+  rewrite Str_app_assoc in H0.
+  apply H0.
+Qed.
+
+
+Module TM1.
+Definition tm := Eval compute in (TM_from_str "1RB0LB_0RC1RF_1LD1RE_0LA0RB_0RD0LA_1LA---").
+Notation "c -->* c'" := (c -[ tm ]->* c') (at level 40).
+Notation "c -->+ c'" := (c -[ tm ]->+ c') (at level 40).
+
+Notation h0 := ((E,<[1]),(B,[0])).
+Notation h1 := ((D,<[1;0]),(B,[0])).
+Notation h2 := ((B,<[1;0;0]),(B,[0])).
+
+Definition f1 (w:seg)(h:head):option((list seg)*(list head)) :=
+List.find (fun '(x,y) => eqb x (h,w)) (
+((h0,[0;1;0;1]),([[0;1;0;1]],[h0;h0]))::
+((h0,[1;0;1]),([[0;0;1]],[]))::
+((h0,[0;0;1]),([[1;0;1]],[h0]))::
+((h2,[0;1;0;1]),([[0;1;0;1]],[h2;h0]))::
+((h2,[0;0;1]),([[0;1;0;1];[0]],[]))::
+((h2,[1;0;1]),([[1];[0;1;0;1]],[]))::
+((h0,[0]),([],[h1]))::
+((h1,[1;0;1]),([[0;1;0;1]],[h0;h0]))::
+((h1,[0;0;1]),([[1;0;1];[1]],[]))::
+((h1,[0;1;0;1]),([[1;0;1]],[h2]))::
+((h0,[1]),([[0]],[]))::
+nil) &&& (fun '(x,y) => Some y).
+
+Definition f0 (w:seg)(h:head):option((list seg)*seg) :=
+List.find (fun '(x,y) => eqb x (h,w)) (
+((h0,[]),([[1;0;1]],[]))::
+((h1,[]),([[1;0;1]],[]))::
+nil) &&& (fun '(x,y) => Some y).
+
+Definition f2 (w:seg)(h:head):option(N*N*head) :=
+List.find (fun '(x,y) => eqb x (h,w)) (
+((h0,[0;1;0;1]),(0%N,1%N,h0))::
+((h0,[1;0;1]),(1%N,0%N,h0))::
+((h0,[0;0;1]),(1%N,0%N,h0))::
+nil) &&& (fun '(x,y) => Some y).
+
+Definition ws_init:(list seg)*seg := ([[0;1;0;1];[0;1;0;1];[0;0;1];[1;0;1]],[]).
+
+Definition hs_step:(list head) := [h2]^^132.
+
+Lemma nonhalt: ~halts tm c0.
+Proof.
+  eapply decide_nonhalt_spec with
+  (tm:=tm) (f2:=f2) (f1:=f1) (f0:=f0) (hs_step:=hs_step) (ws_init:=ws_init)
+  (lh:=0inf<*<[1;0]) (pp:=5%nat) (T:=N.to_nat (10^6)).
+  - intros.
+    unfold f2 in H.
+    apply find_spec in H.
+    gen w h a0 a1 h'.
+    apply f2_spec' with (T:=(10^3)).
+    time vm_compute; reflexivity.
+  - intros.
+    unfold f1 in H.
+    apply find_spec in H.
+    gen w h ws hs.
+    apply f1_spec' with (T:=(10^3)).
+    time vm_compute; reflexivity.
+  - intros.
+    unfold f0 in H.
+    apply find_spec in H.
+    gen w h w'.
+    apply f0_spec' with (T:=(10^3)).
+    time vm_compute; reflexivity.
+  - reflexivity.
+  - intro X; inverts X.
+  - apply BoundedConfig.sideRLs_c_spec with (T:=10^4); reflexivity.
+  - esx.
+  - native_check_eq.
+Time Qed.
+End TM1.
+
+
+Module TM2.
+Definition tm := Eval compute in (TM_from_str "1RB0LB_0RC0RF_1LD1RE_0LA0RB_0RD0LA_1LC---").
+Notation "c -->* c'" := (c -[ tm ]->* c') (at level 40).
+Notation "c -->+ c'" := (c -[ tm ]->+ c') (at level 40).
+
+Notation h0 := ((E,<[0;1]),(A,[0;1])).
+Notation h1 := ((D,<[0;1;0]),(A,[0;1])).
+Notation h2 := ((B,<[0;1;0;0]),(A,[0;1])).
+
+Definition f1 (w:seg)(h:head):option((list seg)*(list head)) :=
+List.find (fun '(x,y) => eqb x (h,w)) (
+((h0,[0;1;0;1]),([[0;1;0;1]],[h0;h0]))::
+((h0,[1;0;1]),([[0;0;1]],[]))::
+((h0,[0;0;1]),([[1;0;1]],[h0]))::
+((h2,[0;1;0;1]),([[0;1;0;1]],[h2;h0]))::
+((h2,[0;0;1]),([[0;1;0;1];[0]],[]))::
+((h2,[1;0;1]),([[1];[0;1;0;1]],[]))::
+((h0,[0]),([],[h1]))::
+((h1,[1;0;1]),([[0;1;0;1]],[h0;h0]))::
+((h1,[0;0;1]),([[1;0;1];[1]],[]))::
+((h1,[0;1;0;1]),([[1;0;1]],[h2]))::
+((h0,[1]),([[0]],[]))::
+nil) &&& (fun '(x,y) => Some y).
+
+Definition f0 (w:seg)(h:head):option((list seg)*seg) :=
+List.find (fun '(x,y) => eqb x (h,w)) (
+((h0,[]),([[1;0;1]],[]))::
+((h1,[]),([[1;0;1]],[]))::
+nil) &&& (fun '(x,y) => Some y).
+
+Definition f2 (w:seg)(h:head):option(N*N*head) :=
+List.find (fun '(x,y) => eqb x (h,w)) (
+((h0,[0;1;0;1]),(0%N,1%N,h0))::
+((h0,[1;0;1]),(1%N,0%N,h0))::
+((h0,[0;0;1]),(1%N,0%N,h0))::
+nil) &&& (fun '(x,y) => Some y).
+
+Definition ws_init:(list seg)*seg := ([[0;1;0;1];[0;1;0;1];[0;0;1];[1;0;1]],[]).
+
+Definition hs_step:(list head) := [h2]^^132.
+
+Lemma nonhalt: ~halts tm c0.
+Proof.
+  eapply decide_nonhalt_spec with
+  (tm:=tm) (f2:=f2) (f1:=f1) (f0:=f0) (hs_step:=hs_step) (ws_init:=ws_init)
+  (lh:=0inf<*<[1]) (pp:=5%nat) (T:=N.to_nat (10^6)).
+  - intros.
+    unfold f2 in H.
+    apply find_spec in H.
+    gen w h a0 a1 h'.
+    apply f2_spec' with (T:=(10^3)).
+    time vm_compute; reflexivity.
+  - intros.
+    unfold f1 in H.
+    apply find_spec in H.
+    gen w h ws hs.
+    apply f1_spec' with (T:=(10^3)).
+    time vm_compute; reflexivity.
+  - intros.
+    unfold f0 in H.
+    apply find_spec in H.
+    gen w h w'.
+    apply f0_spec' with (T:=(10^3)).
+    time vm_compute; reflexivity.
+  - reflexivity.
+  - intro X; inverts X.
+  - apply BoundedConfig.sideRLs_c_spec with (T:=10^4); reflexivity.
+  - esx.
+  - native_check_eq.
+Time Qed.
+End TM2.
+
+
+Module TM3.
+Definition tm := Eval compute in (TM_from_str "1LB0RD_0LC---_1RD0LF_0RE0LF_0LA1RF_0RA1RB").
+Notation "c -->* c'" := (c -[ tm ]->* c') (at level 40).
+Notation "c -->+ c'" := (c -[ tm ]->+ c') (at level 40).
+
+Notation h0 := ((A,<[1;0]),(F,[0;0])).
+Notation h1 := ((D,<[1;0;0]),(F,[0;0])).
+Notation h2 := ((E,<[1;0;0;0]),(F,[0;0])).
+
+Definition f1 (w:seg)(h:head):option((list seg)*(list head)) :=
+List.find (fun '(x,y) => eqb x (h,w)) (
+((h0,[1;0;1;0]),([[1;0;1;0]],[h0;h0]))::
+((h0,[0;1;0]),([[1;1;0]],[]))::
+((h0,[1;1;0]),([[0;1;0]],[h0]))::
+((h2,[1;0;1;0]),([[1;0;1;0]],[h2;h0]))::
+((h2,[1;1;0]),([[1;0;1;0];[1]],[]))::
+((h0,[1]),([],[h1]))::
+((h1,[1;0;1;0]),([[0;1;0]],[h2]))::
+((h1,[1;1;0]),([[0;1;0];[0]],[]))::
+((h0,[0]),([[1]],[]))::
+((h1,[0;1;0]),([[1;0;1;0]],[h0;h0]))::
+((h2,[0;1;0]),([[0;1;0]],[h2]))::
+nil) &&& (fun '(x,y) => Some y).
+
+Definition f0 (w:seg)(h:head):option((list seg)*seg) :=
+List.find (fun '(x,y) => eqb x (h,w)) (
+((h1,[1]),([[0;1;0]],[1]))::
+((h0,[1]),([[0;1;0]],[1]))::
+nil) &&& (fun '(x,y) => Some y).
+
+Definition f2 (w:seg)(h:head):option(N*N*head) :=
+List.find (fun '(x,y) => eqb x (h,w)) (
+((h0,[1;0;1;0]),(0%N,1%N,h0))::
+((h0,[0;1;0]),(1%N,0%N,h0))::
+((h0,[1;1;0]),(1%N,0%N,h0))::
+((h2,[0;1;0]),(0%N,0%N,h2))::
+nil) &&& (fun '(x,y) => Some y).
+
+Definition ws_init:(list seg)*seg := ([[1;0;1;0];[1;0;1;0];[1;0;1;0];[1;0;1;0];[1;0;1;0];[1;1;0];[1;0;1;0];[1;0;1;0];[1;1;0];[1;1;0];[1;1;0];[1;1;0];[1;1;0]],[1]).
+
+Definition hs_step:(list head) := [h2]^^(141*4).
+
+Lemma nonhalt: ~halts tm c0.
+Proof.
+  eapply decide_nonhalt_spec with
+  (tm:=tm) (f2:=f2) (f1:=f1) (f0:=f0) (hs_step:=hs_step) (ws_init:=ws_init)
+  (lh:=0inf<*<[1;0]) (pp:=4%nat) (T:=N.to_nat (10^6)).
+  - intros.
+    unfold f2 in H.
+    apply find_spec in H.
+    gen w h a0 a1 h'.
+    apply f2_spec' with (T:=(10^3)).
+    time vm_compute; reflexivity.
+  - intros.
+    unfold f1 in H.
+    apply find_spec in H.
+    gen w h ws hs.
+    apply f1_spec' with (T:=(10^3)).
+    time vm_compute; reflexivity.
+  - intros.
+    unfold f0 in H.
+    apply find_spec in H.
+    gen w h w'.
+    apply f0_spec' with (T:=(10^3)).
+    time vm_compute; reflexivity.
+  - reflexivity.
+  - intro X; inverts X.
+  - apply BoundedConfig.sideRLs_c_spec with (T:=10^4); reflexivity.
+  - esx.
+  - native_check_eq.
+Time Qed.
+End TM3.
+
+
+Module TM4.
+Definition tm := Eval compute in (TM_from_str "1RB0LB_0RC0LE_1RD0RC_1LB0RE_0LA1RF_0LD---").
+Notation "c -->* c'" := (c -[ tm ]->* c') (at level 40).
+Notation "c -->+ c'" := (c -[ tm ]->+ c') (at level 40).
+
+Notation h0 := ((D,<[0;1]),(A,[0;0])).
+Notation h1 := ((E,<[0;1;0]),(A,[0;0])).
+Notation h2 := ((C,<[0;1;1;0]),(A,[0;0])).
+
+Definition f1 (w:seg)(h:head):option((list seg)*(list head)) :=
+List.find (fun '(x,y) => eqb x (h,w)) (
+((h0,[1;0;1;0]),([[1;0;1;0]],[h0;h0]))::
+((h0,[0;0;0]),([[1;0;0]],[]))::
+((h0,[1;0;0]),([[0;0;0]],[h0]))::
+((h2,[1;0;1;0]),([[1;0;1;0]],[h2;h0]))::
+((h2,[0;0;0]),([[0;0;0];[1;0]],[]))::
+((h0,[1;0]),([],[h2]))::
+((h2,[1;0;0]),([[1;0;1;0]],[h1]))::
+((h1,[1;0;0]),([[1;0;1;0]],[h0]))::
+((h1,[0;0;0]),([[0;0;0];[1]],[]))::
+((h0,[1]),([],[h1]))::
+((h1,[1;0;1;0]),([[1;0;0];[0;0]],[h0;h0]))::
+((h0,[0;0]),([[1;0]],[]))::
+nil) &&& (fun '(x,y) => Some y).
+
+Definition f0 (w:seg)(h:head):option((list seg)*seg) :=
+List.find (fun '(x,y) => eqb x (h,w)) (
+((h0,[]),([[1;0;0]],[]))::
+nil) &&& (fun '(x,y) => Some y).
+
+Definition f2 (w:seg)(h:head):option(N*N*head) :=
+List.find (fun '(x,y) => eqb x (h,w)) (
+((h0,[1;0;1;0]),(0%N,1%N,h0))::
+((h0,[0;0;0]),(1%N,0%N,h0))::
+((h0,[1;0;0]),(1%N,0%N,h0))::
+nil) &&& (fun '(x,y) => Some y).
+
+Definition ws_init:(list seg)*seg := ([[1;0;1;0];[1;0;1;0];[1;0;1;0];[1;0;1;0];[1;0;1;0];[0;0;0];[0;0;0];[0;0;0];[1;0;0];[1;0;0]],[]).
+
+Definition hs_step:(list head) := [h2]^^368.
+
+Lemma nonhalt: ~halts tm c0.
+Proof.
+  eapply decide_nonhalt_spec with
+  (tm:=tm) (f2:=f2) (f1:=f1) (f0:=f0) (hs_step:=hs_step) (ws_init:=ws_init)
+  (lh:=0inf<*<[1]) (pp:=6%nat) (T:=N.to_nat (10^6)).
+  - intros.
+    unfold f2 in H.
+    apply find_spec in H.
+    gen w h a0 a1 h'.
+    apply f2_spec' with (T:=(10^3)).
+    time vm_compute; reflexivity.
+  - intros.
+    unfold f1 in H.
+    apply find_spec in H.
+    gen w h ws hs.
+    apply f1_spec' with (T:=(10^3)).
+    time vm_compute; reflexivity.
+  - intros.
+    unfold f0 in H.
+    apply find_spec in H.
+    gen w h w'.
+    apply f0_spec' with (T:=(10^3)).
+    time vm_compute; reflexivity.
+  - reflexivity.
+  - intro X; inverts X.
+  - apply BoundedConfig.sideRLs_c_spec with (T:=10^4); reflexivity.
+  - esx.
+  - native_check_eq.
+Time Qed.
+End TM4.
+
+
+Module TM5.
+Definition tm := Eval compute in (TM_from_str "1RB0LB_0RC0LE_1RD0RF_1LB0RE_0LA1RB_0LB---").
+Notation "c -->* c'" := (c -[ tm ]->* c') (at level 40).
+Notation "c -->+ c'" := (c -[ tm ]->+ c') (at level 40).
+
+Notation h0 := ((D,<[0;1]),(A,[0;0])).
+Notation h1 := ((E,<[0;1;0]),(A,[0;0])).
+Notation h2 := ((C,<[0;1;1;0]),(A,[0;0])).
+
+Definition f1 (w:seg)(h:head):option((list seg)*(list head)) :=
+List.find (fun '(x,y) => eqb x (h,w)) (
+((h0,[1;0;1;0]),([[1;0;1;0]],[h0;h0]))::
+((h0,[0;0;0]),([[1;0;0]],[]))::
+((h0,[1;0;0]),([[0;0;0]],[h0]))::
+((h2,[1;0;1;0]),([[1;0;1;0]],[h2;h0]))::
+((h2,[0;0;0]),([[0;0;0];[1;0]],[]))::
+((h0,[1;0]),([],[h2]))::
+((h2,[1;0;0]),([[1;0;1;0]],[h1]))::
+((h1,[1;0;0]),([[1;0;1;0]],[h0]))::
+((h1,[0;0;0]),([[0;0;0];[1]],[]))::
+((h0,[1]),([],[h1]))::
+((h1,[1;0;1;0]),([[1;0;0];[0;0]],[h0;h0]))::
+((h0,[0;0]),([[1;0]],[]))::
+nil) &&& (fun '(x,y) => Some y).
+
+Definition f0 (w:seg)(h:head):option((list seg)*seg) :=
+List.find (fun '(x,y) => eqb x (h,w)) (
+((h0,[]),([[1;0;0]],[]))::
+nil) &&& (fun '(x,y) => Some y).
+
+Definition f2 (w:seg)(h:head):option(N*N*head) :=
+List.find (fun '(x,y) => eqb x (h,w)) (
+((h0,[1;0;1;0]),(0%N,1%N,h0))::
+((h0,[0;0;0]),(1%N,0%N,h0))::
+((h0,[1;0;0]),(1%N,0%N,h0))::
+nil) &&& (fun '(x,y) => Some y).
+
+Definition ws_init:(list seg)*seg := ([[1;0;1;0];[1;0;1;0];[1;0;1;0];[1;0;1;0];[1;0;1;0];[0;0;0];[0;0;0];[0;0;0];[1;0;0];[1;0;0]],[]).
+
+Definition hs_step:(list head) := [h2]^^368.
+
+Lemma nonhalt: ~halts tm c0.
+Proof.
+  eapply decide_nonhalt_spec with
+  (tm:=tm) (f2:=f2) (f1:=f1) (f0:=f0) (hs_step:=hs_step) (ws_init:=ws_init)
+  (lh:=0inf<*<[1]) (pp:=6%nat) (T:=N.to_nat (10^6)).
+  - intros.
+    unfold f2 in H.
+    apply find_spec in H.
+    gen w h a0 a1 h'.
+    apply f2_spec' with (T:=(10^3)).
+    time vm_compute; reflexivity.
+  - intros.
+    unfold f1 in H.
+    apply find_spec in H.
+    gen w h ws hs.
+    apply f1_spec' with (T:=(10^3)).
+    time vm_compute; reflexivity.
+  - intros.
+    unfold f0 in H.
+    apply find_spec in H.
+    gen w h w'.
+    apply f0_spec' with (T:=(10^3)).
+    time vm_compute; reflexivity.
+  - reflexivity.
+  - intro X; inverts X.
+  - apply BoundedConfig.sideRLs_c_spec with (T:=10^4); reflexivity.
+  - esx.
+  - native_check_eq.
+Time Qed.
+End TM5.
+
+
+Module TM6.
+Definition tm := Eval compute in (TM_from_str "1RB0LB_0RC0LE_1RD0RF_1LB0RE_0LA0RE_0LB---").
+Notation "c -->* c'" := (c -[ tm ]->* c') (at level 40).
+Notation "c -->+ c'" := (c -[ tm ]->+ c') (at level 40).
+
+Notation h0 := ((D,<[0;1]),(A,[0;0])).
+Notation h1 := ((E,<[0;1;0]),(A,[0;0])).
+Notation h2 := ((C,<[0;1;1;0]),(A,[0;0])).
+
+Definition f1 (w:seg)(h:head):option((list seg)*(list head)) :=
+List.find (fun '(x,y) => eqb x (h,w)) (
+((h0,[1;0;1;0]),([[1;0;1;0]],[h0;h0]))::
+((h0,[0;0;0]),([[1;0;0]],[]))::
+((h0,[1;0;0]),([[0;0;0]],[h0]))::
+((h2,[1;0;1;0]),([[1;0;1;0]],[h2;h0]))::
+((h2,[0;0;0]),([[0;0;0];[1;0]],[]))::
+((h0,[1;0]),([],[h2]))::
+((h2,[1;0;0]),([[1;0;1;0]],[h1]))::
+((h1,[1;0;0]),([[1;0;1;0]],[h0]))::
+((h1,[0;0;0]),([[0;0;0];[1]],[]))::
+((h0,[1]),([],[h1]))::
+((h1,[1;0;1;0]),([[1;0;0];[0;0]],[h0;h0]))::
+((h0,[0;0]),([[1;0]],[]))::
+nil) &&& (fun '(x,y) => Some y).
+
+Definition f0 (w:seg)(h:head):option((list seg)*seg) :=
+List.find (fun '(x,y) => eqb x (h,w)) (
+((h0,[]),([[1;0;0]],[]))::
+nil) &&& (fun '(x,y) => Some y).
+
+Definition f2 (w:seg)(h:head):option(N*N*head) :=
+List.find (fun '(x,y) => eqb x (h,w)) (
+((h0,[1;0;1;0]),(0%N,1%N,h0))::
+((h0,[0;0;0]),(1%N,0%N,h0))::
+((h0,[1;0;0]),(1%N,0%N,h0))::
+nil) &&& (fun '(x,y) => Some y).
+
+Definition ws_init:(list seg)*seg := ([[1;0;1;0];[1;0;1;0];[1;0;1;0];[1;0;1;0];[1;0;1;0];[0;0;0];[0;0;0];[0;0;0];[1;0;0];[1;0;0]],[]).
+
+Definition hs_step:(list head) := [h2]^^368.
+
+Lemma nonhalt: ~halts tm c0.
+Proof.
+  eapply decide_nonhalt_spec with
+  (tm:=tm) (f2:=f2) (f1:=f1) (f0:=f0) (hs_step:=hs_step) (ws_init:=ws_init)
+  (lh:=0inf<*<[1]) (pp:=6%nat) (T:=N.to_nat (10^6)).
+  - intros.
+    unfold f2 in H.
+    apply find_spec in H.
+    gen w h a0 a1 h'.
+    apply f2_spec' with (T:=(10^3)).
+    time vm_compute; reflexivity.
+  - intros.
+    unfold f1 in H.
+    apply find_spec in H.
+    gen w h ws hs.
+    apply f1_spec' with (T:=(10^3)).
+    time vm_compute; reflexivity.
+  - intros.
+    unfold f0 in H.
+    apply find_spec in H.
+    gen w h w'.
+    apply f0_spec' with (T:=(10^3)).
+    time vm_compute; reflexivity.
+  - reflexivity.
+  - intro X; inverts X.
+  - apply BoundedConfig.sideRLs_c_spec with (T:=10^4); reflexivity.
+  - esx.
+  - native_check_eq.
+Time Qed.
+End TM6.
+
+
+Module TM7.
+Definition tm := Eval compute in (TM_from_str "1RB0LB_0RC0LE_1RD0RF_1LB0RE_0LA1RB_1RE---").
+Notation "c -->* c'" := (c -[ tm ]->* c') (at level 40).
+Notation "c -->+ c'" := (c -[ tm ]->+ c') (at level 40).
+
+Notation h0 := ((D,<[0;1]),(A,[0;0])).
+Notation h1 := ((C,<[0;1;1;0]),(A,[0;0;1;0])).
+Notation h2 := ((E,<[0;1;0]),(A,[0;0])).
+Notation h3 := ((C,<[0;1;1;0]),(A,[0;0])).
+Notation h4 := ((E,<[0;1;1;0;0;1]),(A,[0;0;1;0])).
+Notation h5 := ((E,<[0;1;1;1;0;1;0]),(A,[0;0;1;0])).
+Notation h6 := ((E,<[0;1;1;0;0;1]),(A,[0;0])).
+Notation h7 := ((D,<[0;1;0;1;0;1]),(A,[0;0])).
+Notation h8 := ((E,<[0;1;1;1;0;1;0]),(A,[0;0])).
+
+Definition f1 (w:seg)(h:head):option((list seg)*(list head)) :=
+List.find (fun '(x,y) => eqb x (h,w)) (
+((h1,[1;0;1;0]),([[1;0;1;0]],[h1;h1]))::
+((h1,[1;0;0;0;0]),([[1;0;0;0;0]],[h0]))::
+((h1,[1;0;1;0;0]),([[1;0;1;0;0]],[h0]))::
+((h0,[0;0;0]),([[1;0;0]],[]))::
+((h0,[1;0;0]),([[0;0;0]],[h0]))::
+((h0,[1;0;1;0;1;0]),([[1;0;1;0;1;0]],[h1;h1]))::
+((h4,[1;0;1;0]),([[1;0;1;0]],[h4;h1]))::
+((h4,[1;0;0;0;0]),([[1;0;1;0;0];[1;0]],[]))::
+((h4,[1;0;1;0;0]),([[1;0;1;0]],[h5;h1]))::
+((h0,[1;0]),([],[h3]))::
+((h3,[0;0;0]),([[0;0;0];[1;0]],[]))::
+((h3,[1;0;0]),([],[h8]))::
+((h8,[1;0;0]),([[1;0;1;0;1;0];[1;0]],[h0]))::
+((h1,[1;0]),([],[h4]))::
+((h4,[1;0;0]),([[1;0;1;0;0]],[h0]))::
+((h5,[0;0;0]),([[1;0;0;0;0];[1]],[]))::
+((h0,[1]),([],[h2]))::
+((h2,[0;0;0]),([[0;0;0];[1]],[]))::
+((h2,[1;0;1;0;1;0]),([[1;0;0];[0;0;1;0]],[h1;h1]))::
+((h0,[0;0;1;0]),([[1;0;1;0]],[]))::
+((h0,[1;0;1;0]),([],[h6]))::
+((h6,[1;0;1;0;0]),([[1;0;1;0;1;0]],[h5;h1]))::
+((h2,[1;0;0]),([],[h7]))::
+((h7,[1;0;0]),([[1;0;1;0;0;0;0]],[h0]))::
+((h0,[1;0;1;0;0;0;0]),([[1;0;1;0;0;0;0]],[h0]))::
+((h8,[1;0;1;0;1;0]),([[1;0;1;0;1;0;0;0;0;1;0]],[h1;h1]))::
+((h0,[1;0;1;0;1;0;0;0;0;1;0]),([[1;0;1;0;1;0;0;1;0;1;0]],[]))::
+((h0,[1;0;1;0;1;0;0;1;0;1;0]),([[1;0;1;0;1;0;0];[1;0]],[h4]))::
+((h0,[1;0;1;0;1;0;0]),([[1;0;1;0;1;0;0]],[h0]))::
+((h3,[1;0;1;0;0]),([[1;0;1;0;1;0;0]],[h0]))::
+((h3,[1;0;1;0;0;0;0]),([[1;0;1;0;1;0;0;1;0]],[]))::
+((h0,[1;0;1;0;1;0;0;1;0]),([[1;0;1;0;1;0;0]],[h3]))::
+((h8,[0;0;0]),([[1;0;1;0;0;0;0];[1]],[]))::
+((h2,[1;0;1;0;1;0;0]),([[1;0;0];[0;0;1;0;0]],[h0]))::
+((h0,[0;0;1;0;0]),([[1;0;1;0;0]],[]))::
+((h0,[1;0;1;0;0]),([],[h8]))::
+((h8,[1;0;1;0;1;0;0]),([[1;0;1;0;1;0;0;0;0;1;0;0]],[h0]))::
+((h0,[1;0;1;0;1;0;0;0;0;1;0;0]),([[1;0;1;0;1;0;0;1;0;1;0;0]],[]))::
+((h0,[1;0;1;0;1;0;0;1;0;1;0;0]),([[1;0;1;0;1;0;0];[1;0;1;0]],[h2]))::
+((h6,[1;0;0]),([[1;0;1;0;1;0;0]],[h0]))::
+((h8,[1;0;1;0;0;0;0]),([[1;0;1;0;1;0;0];[0;0;0];[0;0]],[h0]))::
+((h0,[0;0]),([[1;0]],[]))::
+((h4,[0;0;0]),([[1;0;0;0;0]],[h0]))::
+((h6,[0;0;0]),([[1;0;1;0;0;0;0]],[h0]))::
+((h6,[1;0;0;0;0]),([[1;0;1;0;1;0;0];[1;0]],[]))::
+((h5,[1;0;1;0;1;0;0]),([[1;0;1;0;0];[0;0;1;0;0]],[h0]))::
+((h3,[1;0;1;0;1;0;0]),([[1;0;1;0;1;0]],[h5;h1]))::
+((h5,[1;0;1;0;0;0;0]),([[1;0;1;0;0];[0;0;0];[0;0]],[h0]))::
+((h4,[1;0;1;0;1;0]),([[1;0;1;0];[1;0;1;0]],[h1;h1;h1;h1]))::
+((h2,[1;0;1;0;0;0;0]),([[1;0;0];[0;0;0];[0;0]],[h0]))::
+((h7,[1;0;1;0;1;0]),([[1;0;1;0;1;0];[1;0;1;0]],[h1;h1]))::
+((h6,[1;0;1;0;1;0]),([[1;0;1;0;1;0];[1;0;1;0]],[h1;h1;h1;h1]))::
+((h5,[1;0;0]),([[1;0;1;0];[1;0]],[h0]))::
+((h4,[1;0;1;0;1;0;0]),([[1;0;1;0];[1;0;1;0;0]],[h0;h0]))::
+((h3,[1;0;1;0]),([[1;0;1;0;1;0]],[h1;h1]))::
+((h3,[1;0;1;0;1;0]),([[1;0;1;0;1;0]],[h4;h1]))::
+((h5,[1;0;1;0;1;0]),([[1;0;1;0;0];[0;0;1;0]],[h1;h1]))::
+((h6,[1;0;1;0]),([[1;0;1;0;1;0]],[h4;h1]))::
+((h4,[1;0;1;0;0;0;0]),([[1;0;1;0];[1;0;0;0;0]],[h0;h0]))::
+((h6,[1;0;1;0;0;0;0]),([[1;0;1;0;1;0];[1;0;0;0;0]],[h0;h0]))::
+((h7,[0;0;0]),([[1;0;1;0;1;0;0]],[]))::
+((h7,[1;0;1;0;0;0;0]),([[1;0;1;0;1;0];[1;0;0;0;0]],[h0]))::
+((h7,[1;0;1;0;1;0;0]),([[1;0;1;0;1;0];[1;0;1;0;0]],[h0]))::
+((h6,[1;0;1;0;1;0;0]),([[1;0;1;0;1;0];[1;0;1;0;0]],[h0;h0]))::
+nil) &&& (fun '(x,y) => Some y).
+
+Definition f0 (w:seg)(h:head):option((list seg)*seg) :=
+List.find (fun '(x,y) => eqb x (h,w)) (
+((h0,[]),([[1;0;0]],[]))::
+nil) &&& (fun '(x,y) => Some y).
+
+Definition f2 (w:seg)(h:head):option(N*N*head) :=
+List.find (fun '(x,y) => eqb x (h,w)) (
+((h1,[1;0;1;0]),(0%N,1%N,h1))::
+((h1,[1;0;0;0;0]),(0%N,0%N,h0))::
+((h1,[1;0;1;0;0]),(0%N,0%N,h0))::
+((h0,[0;0;0]),(1%N,0%N,h0))::
+((h0,[1;0;0]),(1%N,0%N,h0))::
+((h0,[1;0;1;0;1;0]),(0%N,1%N,h1))::
+((h0,[1;0;1;0;0;0;0]),(0%N,0%N,h0))::
+((h0,[1;0;1;0;1;0;0]),(0%N,0%N,h0))::
+nil) &&& (fun '(x,y) => Some y).
+
+Definition ws_init:(list seg)*seg := ([[1;0;1;0];[1;0;1;0];[1;0;1;0];[1;0;1;0];[1;0;0;0;0];[0;0;0];[0;0;0];[1;0;0];[1;0;0]],[]).
+
+Definition hs_step:(list head) := [h4]^^368.
+
+
+Lemma nonhalt: ~halts tm c0.
+Proof.
+  eapply decide_nonhalt_spec with
+  (tm:=tm) (f2:=f2) (f1:=f1) (f0:=f0) (hs_step:=hs_step) (ws_init:=ws_init)
+  (lh:=0inf<*<[1]) (pp:=6%nat) (T:=N.to_nat (10^6)).
+  - intros.
+    unfold f2 in H.
+    apply find_spec in H.
+    gen w h a0 a1 h'.
+    apply f2_spec' with (T:=(10^3)).
+    time vm_compute; reflexivity.
+  - intros.
+    unfold f1 in H.
+    apply find_spec in H.
+    gen w h ws hs.
+    apply f1_spec' with (T:=(10^3)).
+    time vm_compute; reflexivity.
+  - intros.
+    unfold f0 in H.
+    apply find_spec in H.
+    gen w h w'.
+    apply f0_spec' with (T:=(10^3)).
+    time vm_compute; reflexivity.
+  - reflexivity.
+  - intro X; inverts X.
+  - apply BoundedConfig.sideRLs_c_spec with (T:=10^4); reflexivity.
+  - esx.
+  - native_check_eq.
+Time Qed.
+End TM7.
+
+
+Module TM8.
+Definition tm := Eval compute in (TM_from_str "1RB---_1LC0RC_0RE0LD_0RE1LB_0LB1RF_1RB0RA").
+Notation "c -->* c'" := (c -[ tm ]->* c') (at level 40).
+Notation "c -->+ c'" := (c -[ tm ]->+ c') (at level 40).
+
+Notation h0 := ((B,<[]),(C,[])).
+Notation h1 := ((C,<[0]),(C,[])).
+Notation h2 := ((E,<[0;0]),(C,[])).
+
+Definition f1 (w:seg)(h:head):option((list seg)*(list head)) :=
+List.find (fun '(x,y) => eqb x (h,w)) (
+((h0,[1;0;1;0]),([[1;0;1;0]],[h0;h0]))::
+((h0,[1;1;0]),([[1;0;0]],[]))::
+((h0,[1;0;0]),([[1;1;0]],[h0]))::
+((h2,[1;0;1;0]),([[1;0;1;0]],[h2;h0]))::
+((h2,[1;1;0]),([[1;1;0]],[h0;h2]))::
+((h2,[1;0;0]),([[1;0;1;0]],[h1]))::
+((h0,[1;0]),([],[h2]))::
+((h1,[1;0;1;0]),([[1;0;0];[1;0]],[]))::
+((h1,[1;1;0]),([[1;0;1;0]],[]))::
+((h1,[1;0;0]),([[1;0;0];[0]],[]))::
+((h0,[0]),([[1]],[]))::
+((h0,[1]),([],[h1]))::
+nil) &&& (fun '(x,y) => Some y).
+
+Definition f0 (w:seg)(h:head):option((list seg)*seg) :=
+List.find (fun '(x,y) => eqb x (h,w)) (
+((h0,[]),([[1;0;0]],[]))::
+nil) &&& (fun '(x,y) => Some y).
+
+Definition f2 (w:seg)(h:head):option(N*N*head) :=
+List.find (fun '(x,y) => eqb x (h,w)) (
+((h0,[1;0;1;0]),(0%N,1%N,h0))::
+((h0,[1;1;0]),(1%N,0%N,h0))::
+((h0,[1;0;0]),(1%N,0%N,h0))::
+nil) &&& (fun '(x,y) => Some y).
+
+Definition ws_init:(list seg)*seg := ([[1;0;1;0];[1;0;1;0];[1;0;1;0];[1;0;1;0];[1;0;1;0];[1;0;1;0];[1;0;0];[1;1;0];[1;1;0];[1;1;0];[1;1;0];[1;0;0];[1;0;0]],[]).
+
+Definition hs_step:(list head) := [h2;h0]^^108.
+
+
+Lemma nonhalt: ~halts tm c0.
+Proof.
+  eapply decide_nonhalt_spec with
+  (tm:=tm) (f2:=f2) (f1:=f1) (f0:=f0) (hs_step:=hs_step) (ws_init:=ws_init)
+  (lh:=0inf<*<[1;1]) (pp:=6%nat) (T:=N.to_nat (10^6)).
+  - intros.
+    unfold f2 in H.
+    apply find_spec in H.
+    gen w h a0 a1 h'.
+    apply f2_spec' with (T:=(10^3)).
+    time vm_compute; reflexivity.
+  - intros.
+    unfold f1 in H.
+    apply find_spec in H.
+    gen w h ws hs.
+    apply f1_spec' with (T:=(10^3)).
+    time vm_compute; reflexivity.
+  - intros.
+    unfold f0 in H.
+    apply find_spec in H.
+    gen w h w'.
+    apply f0_spec' with (T:=(10^3)).
+    time vm_compute; reflexivity.
+  - reflexivity.
+  - intro X; inverts X.
+  - apply BoundedConfig.sideRLs_c_spec with (T:=10^4); reflexivity.
+  - esx.
+  - native_check_eq.
+Time Qed.
+End TM8.
+
+
+Module TM9.
+Definition tm := Eval compute in (TM_from_str "1RB---_0LC0RF_1RB0RD_0LE0RA_1LF1RC_1RE0LD").
+Notation "c -->* c'" := (c -[ tm ]->* c') (at level 40).
+Notation "c -->+ c'" := (c -[ tm ]->+ c') (at level 40).
+
+Notation h0 := ((E,<[1;0;1]),(D,[0;1;0])).
+Notation h1 := ((C,<[1;0;1;1]),(D,[0;1;0])).
+Notation h2 := ((B,<[1;0;1;1;1]),(D,[0;1;0])).
+Notation h3 := ((B,<[1;0;1;1;0;0;1]),(D,[0;1;0])).
+
+Definition f1 (w:seg)(h:head):option((list seg)*(list head)) :=
+List.find (fun '(x,y) => eqb x (h,w)) (
+((h0,[1;0;1;0]),([[1;0;1;0]],[h0;h0]))::
+((h0,[0;1;0]),([[1;1;0]],[]))::
+((h0,[1;1;0]),([[0;1;0]],[h0]))::
+((h2,[1;0;1;0]),([[1;0;1;0]],[h2;h0]))::
+((h2,[1;1;0]),([[1;0;1;0];[1]],[]))::
+((h2,[0;1;0]),([[0;1;0]],[h2]))::
+((h1,[1;0;1;0]),([[0;1;0]],[h2]))::
+((h1,[1;1;0]),([],[h3]))::
+((h1,[0;1;0]),([[1;0;1;0]],[h0;h0]))::
+((h3,[0;1;0]),([[0;1;0];[1;0;1;0]],[h0;h0;h0;h0]))::
+((h3,[1;1;0]),([[0;1;0];[1;1;0;0]],[]))::
+((h3,[1;0;1;0]),([[0;1;0];[1;1;0]],[h2]))::
+((h0,[1;1;0;0]),([[0;1;0];[1]],[]))::
+((h0,[1]),([],[h1]))::
+nil) &&& (fun '(x,y) => Some y).
+
+Definition f0 (w:seg)(h:head):option((list seg)*seg) :=
+List.find (fun '(x,y) => eqb x (h,w)) (
+((h0,[1]),([[0;1;0]],[1]))::
+nil) &&& (fun '(x,y) => Some y).
+
+Definition f2 (w:seg)(h:head):option(N*N*head) :=
+List.find (fun '(x,y) => eqb x (h,w)) (
+((h0,[1;0;1;0]),(0%N,1%N,h0))::
+((h0,[0;1;0]),(1%N,0%N,h0))::
+((h0,[1;1;0]),(1%N,0%N,h0))::
+((h2,[0;1;0]),(0%N,0%N,h2))::
+nil) &&& (fun '(x,y) => Some y).
+
+Definition ws_init:(list seg)*seg := ([[1;0;1;0];[1;0;1;0];[1;0;1;0];[1;0;1;0];[1;0;1;0];[1;0;1;0];[1;0;1;0];[1;1;0];[1;0;1;0];[1;0;1;0];[1;1;0];[1;0;1;0];[1;1;0];[1;1;0];[0;1;0];[1;1;0];[0;1;0];[0;1;0];[0;1;0];[0;1;0]],[1]).
+
+Definition hs_step:(list head) := [h2]^^172.
+
+Lemma nonhalt: ~halts tm c0.
+Proof.
+  eapply decide_nonhalt_spec with
+  (tm:=tm) (f2:=f2) (f1:=f1) (f0:=f0) (hs_step:=hs_step) (ws_init:=ws_init)
+  (lh:=0inf<*<[]) (pp:=8%nat) (T:=N.to_nat (10^6)).
+  - intros.
+    unfold f2 in H.
+    apply find_spec in H.
+    gen w h a0 a1 h'.
+    apply f2_spec' with (T:=(10^3)).
+    time vm_compute; reflexivity.
+  - intros.
+    unfold f1 in H.
+    apply find_spec in H.
+    gen w h ws hs.
+    apply f1_spec' with (T:=(10^3)).
+    time vm_compute; reflexivity.
+  - intros.
+    unfold f0 in H.
+    apply find_spec in H.
+    gen w h w'.
+    apply f0_spec' with (T:=(10^3)).
+    time vm_compute; reflexivity.
+  - reflexivity.
+  - intro X; inverts X.
+  - apply BoundedConfig.sideRLs_c_spec with (T:=10^4); reflexivity.
+  - esx.
+  - native_check_eq.
+Time Qed.
+End TM9.
+
+
+Module TM10.
+Definition tm := Eval compute in (TM_from_str "1RB0LC_1LA1RD_0LB0RF_1RE0RC_0LD0RA_1RE---").
+Notation "c -->* c'" := (c -[ tm ]->* c') (at level 40).
+Notation "c -->+ c'" := (c -[ tm ]->+ c') (at level 40).
+
+Notation h0 := ((B,<[1;0;1]),(C,[0;1;0])).
+Notation h1 := ((D,<[1;0;1;1]),(C,[0;1;0])).
+Notation h2 := ((E,<[1;0;1;1;1]),(C,[0;1;0])).
+Notation h3 := ((E,<[1;0;1;1;0;0;1]),(C,[0;1;0])).
+
+Definition f1 (w:seg)(h:head):option((list seg)*(list head)) :=
+List.find (fun '(x,y) => eqb x (h,w)) (
+((h0,[1;0;1;0]),([[1;0;1;0]],[h0;h0]))::
+((h0,[0;1;0]),([[1;1;0]],[]))::
+((h0,[1;1;0]),([[0;1;0]],[h0]))::
+((h2,[1;0;1;0]),([[1;0;1;0]],[h2;h0]))::
+((h2,[1;1;0]),([[1;0;1;0];[1]],[]))::
+((h2,[0;1;0]),([[0;1;0]],[h2]))::
+((h1,[1;0;1;0]),([[0;1;0]],[h2]))::
+((h1,[1;1;0]),([],[h3]))::
+((h1,[0;1;0]),([[1;0;1;0]],[h0;h0]))::
+((h3,[0;1;0]),([[0;1;0];[1;0;1;0]],[h0;h0;h0;h0]))::
+((h3,[1;1;0]),([[0;1;0];[1;1;0;0]],[]))::
+((h3,[1;0;1;0]),([[0;1;0];[1;1;0]],[h2]))::
+((h0,[1;1;0;0]),([[0;1;0];[1]],[]))::
+((h0,[1]),([],[h1]))::
+nil) &&& (fun '(x,y) => Some y).
+
+Definition f0 (w:seg)(h:head):option((list seg)*seg) :=
+List.find (fun '(x,y) => eqb x (h,w)) (
+((h0,[1]),([[0;1;0]],[1]))::
+nil) &&& (fun '(x,y) => Some y).
+
+Definition f2 (w:seg)(h:head):option(N*N*head) :=
+List.find (fun '(x,y) => eqb x (h,w)) (
+((h0,[1;0;1;0]),(0%N,1%N,h0))::
+((h0,[0;1;0]),(1%N,0%N,h0))::
+((h0,[1;1;0]),(1%N,0%N,h0))::
+((h2,[0;1;0]),(0%N,0%N,h2))::
+nil) &&& (fun '(x,y) => Some y).
+
+Definition ws_init:(list seg)*seg := ([[1;0;1;0];[1;0;1;0];[1;0;1;0];[1;0;1;0];[1;0;1;0];[1;0;1;0];[1;0;1;0];[1;1;0];[1;0;1;0];[1;0;1;0];[1;1;0];[1;0;1;0];[1;1;0];[1;1;0];[0;1;0];[1;1;0];[0;1;0];[0;1;0];[0;1;0];[0;1;0]],[1]).
+
+Definition hs_step:(list head) := [h2]^^172.
+
+Lemma nonhalt: ~halts tm c0.
+Proof.
+  eapply decide_nonhalt_spec with
+  (tm:=tm) (f2:=f2) (f1:=f1) (f0:=f0) (hs_step:=hs_step) (ws_init:=ws_init)
+  (lh:=0inf<*<[1;0;0]) (pp:=8%nat) (T:=N.to_nat (10^6)).
+  - intros.
+    unfold f2 in H.
+    apply find_spec in H.
+    gen w h a0 a1 h'.
+    apply f2_spec' with (T:=(10^3)).
+    time vm_compute; reflexivity.
+  - intros.
+    unfold f1 in H.
+    apply find_spec in H.
+    gen w h ws hs.
+    apply f1_spec' with (T:=(10^3)).
+    time vm_compute; reflexivity.
+  - intros.
+    unfold f0 in H.
+    apply find_spec in H.
+    gen w h w'.
+    apply f0_spec' with (T:=(10^3)).
+    time vm_compute; reflexivity.
+  - reflexivity.
+  - intro X; inverts X.
+  - apply BoundedConfig.sideRLs_c_spec with (T:=10^4); reflexivity.
+  - esx.
+  - native_check_eq.
+Time Qed.
+End TM10.
+
+
+Module TM11.
+Definition tm := Eval compute in (TM_from_str "1LB0RD_0LC---_1RD0LF_0RE0RE_0LA1RF_0RA1RB").
+Notation "c -->* c'" := (c -[ tm ]->* c') (at level 40).
+Notation "c -->+ c'" := (c -[ tm ]->+ c') (at level 40).
+
+Notation h0 := ((A,<[1;0]),(F,[0;0])).
+Notation h1 := ((D,<[1;0;0]),(F,[0;0])).
+Notation h2 := ((E,<[1;0;0;0]),(F,[0;0])).
+
+Definition f1 (w:seg)(h:head):option((list seg)*(list head)) :=
+List.find (fun '(x,y) => eqb x (h,w)) (
+((h0,[1;0;1;0]),([[1;0;1;0]],[h0;h0]))::
+((h0,[0;1;0]),([[1;1;0]],[]))::
+((h0,[1;1;0]),([[0;1;0]],[h0]))::
+((h2,[1;0;1;0]),([[1;0;1;0]],[h2;h0]))::
+((h2,[0;1;0]),([[0;1;0]],[h2]))::
+((h2,[1;1;0]),([[1;0;1;0];[1]],[]))::
+((h0,[1]),([],[h1]))::
+((h1,[1;0;1;0]),([[0;1;0]],[h2]))::
+((h1,[0;1;0]),([[1;0;1;0]],[h0;h0]))::
+((h1,[1;1;0]),([[1;0;1;0]],[h0;h0]))::
+nil) &&& (fun '(x,y) => Some y).
+
+Definition f0 (w:seg)(h:head):option((list seg)*seg) :=
+List.find (fun '(x,y) => eqb x (h,w)) (
+((h0,[1]),([[0;1;0]],[1]))::
+nil) &&& (fun '(x,y) => Some y).
+
+Definition f2 (w:seg)(h:head):option(N*N*head) :=
+List.find (fun '(x,y) => eqb x (h,w)) (
+((h0,[1;0;1;0]),(0%N,1%N,h0))::
+((h0,[0;1;0]),(1%N,0%N,h0))::
+((h0,[1;1;0]),(1%N,0%N,h0))::
+((h2,[0;1;0]),(0%N,0%N,h2))::
+nil) &&& (fun '(x,y) => Some y).
+
+Definition ws_init:(list seg)*seg := ([[1;0;1;0];[1;0;1;0];[1;0;1;0];[1;0;1;0];[1;0;1;0];[1;1;0];[1;0;1;0];[1;0;1;0];[1;1;0];[1;1;0];[1;1;0];[1;1;0];[1;1;0]],[1]).
+
+Definition hs_step:(list head) := [h2]^^60.
+
+Lemma nonhalt: ~halts tm c0.
+Proof.
+  eapply decide_nonhalt_spec with
+  (tm:=tm) (f2:=f2) (f1:=f1) (f0:=f0) (hs_step:=hs_step) (ws_init:=ws_init)
+  (lh:=0inf<*<[1;0]) (pp:=4%nat) (T:=N.to_nat (10^6)).
+  - intros.
+    unfold f2 in H.
+    apply find_spec in H.
+    gen w h a0 a1 h'.
+    apply f2_spec' with (T:=(10^3)).
+    time vm_compute; reflexivity.
+  - intros.
+    unfold f1 in H.
+    apply find_spec in H.
+    gen w h ws hs.
+    apply f1_spec' with (T:=(10^3)).
+    time vm_compute; reflexivity.
+  - intros.
+    unfold f0 in H.
+    apply find_spec in H.
+    gen w h w'.
+    apply f0_spec' with (T:=(10^3)).
+    time vm_compute; reflexivity.
+  - reflexivity.
+  - intro X; inverts X.
+  - apply BoundedConfig.sideRLs_c_spec with (T:=10^4); reflexivity.
+  - esx.
+  - native_check_eq.
+Time Qed.
+End TM11.
+
+
+Module TM12.
+Definition tm := Eval compute in (TM_from_str "1LB0RC_1RC0LB_0RD1LB_0LA1RE_0RA1RF_0RC---").
+Notation "c -->* c'" := (c -[ tm ]->* c') (at level 40).
+Notation "c -->+ c'" := (c -[ tm ]->+ c') (at level 40).
+
+Notation h0 := ((A,<[1;0]),(B,[0;0])).
+Notation h1 := ((D,<[1;0;0;0]),(B,[0;0])).
+Notation h2 := ((C,<[1;1;0;1;1;0]),(B,[0;0])).
+Notation h3 := ((C,<[1;0;0;0;1;1;0]),(B,[0;0])).
+
+Definition f1 (w:seg)(h:head):option((list seg)*(list head)) :=
+List.find (fun '(x,y) => eqb x (h,w)) (
+((h0,[1;0;1;0]),([[1;0;1;0]],[h0;h0]))::
+((h0,[0;1;0]),([[1;1;0]],[]))::
+((h0,[1;1;0]),([[0;1;0]],[h0]))::
+((h1,[1;0;1;0]),([[1;0;1;0]],[h1;h0]))::
+((h1,[0;1;0]),([[0;1;0]],[h1]))::
+((h1,[1;1;0]),([],[h3]))::
+((h0,[1;0]),([],[h1]))::
+((h3,[1;0;1;0]),([[1;0;1;0];[1;1;0];[1;0]],[]))::
+((h3,[0;1;0]),([[1;0;1;0];[1;0;1;0]],[h0;h0]))::
+((h3,[1;1;0]),([[1;0;1;0];[1;1;1;0]],[]))::
+((h0,[1;1;1;0]),([],[h2]))::
+((h2,[1;0;1;0]),([[0;1;0];[0;1;0];[1;0]],[]))::
+((h2,[1;1;0]),([[0;1;0];[0;1;1;0]],[]))::
+((h2,[0;1;0]),([[0;1;0];[0;0;1;0]],[h0;h0]))::
+((h0,[0;1;1;0]),([[1;1;1;0]],[]))::
+((h0,[0;0;1;0]),([[1;0;1;0]],[]))::
+nil) &&& (fun '(x,y) => Some y).
+
+Definition f0 (w:seg)(h:head):option((list seg)*seg) :=
+List.find (fun '(x,y) => eqb x (h,w)) (
+((h0,[1]),([[0;1;0]],[1]))::
+((h1,[1]),([[1;0;1;0];[0;1;0]],[1]))::
+((h2,[1]),([[0;1;0];[0;1;0]],[]))::
+((h0,[]),([],[1]))::
+nil) &&& (fun '(x,y) => Some y).
+
+Definition f2 (w:seg)(h:head):option(N*N*head) :=
+List.find (fun '(x,y) => eqb x (h,w)) (
+((h0,[1;0;1;0]),(0%N,1%N,h0))::
+((h0,[0;1;0]),(1%N,0%N,h0))::
+((h0,[1;1;0]),(1%N,0%N,h0))::
+((h1,[0;1;0]),(0%N,0%N,h1))::
+nil) &&& (fun '(x,y) => Some y).
+
+Definition ws_init:(list seg)*seg := ([[1;0;1;0];[1;0;1;0];[1;0;1;0];[1;0;1;0];[1;0;1;0];[1;0;1;0];[1;1;0];[1;0;1;0];[1;0;1;0];[0;1;0];[0;1;0];[0;1;0];[0;1;0];[0;1;0];[0;1;0];[0;1;0]],[1]).
+
+Definition hs_step:(list head) := [h1]^^(19*4).
+
+Lemma nonhalt: ~halts tm c0.
+Proof.
+  eapply decide_nonhalt_spec with
+  (tm:=tm) (f2:=f2) (f1:=f1) (f0:=f0) (hs_step:=hs_step) (ws_init:=ws_init)
+  (lh:=0inf<*<[1;0]) (pp:=6%nat) (T:=N.to_nat (10^6)).
+  - intros.
+    unfold f2 in H.
+    apply find_spec in H.
+    gen w h a0 a1 h'.
+    apply f2_spec' with (T:=(10^3)).
+    time vm_compute; reflexivity.
+  - intros.
+    unfold f1 in H.
+    apply find_spec in H.
+    gen w h ws hs.
+    apply f1_spec' with (T:=(10^3)).
+    time vm_compute; reflexivity.
+  - intros.
+    unfold f0 in H.
+    apply find_spec in H.
+    gen w h w'.
+    apply f0_spec' with (T:=(10^3)).
+    time vm_compute; reflexivity.
+  - reflexivity.
+  - intro X; inverts X.
+  - apply BoundedConfig.sideRLs_c_spec with (T:=10^4); reflexivity.
+  - esx.
+  - native_check_eq.
+Time Qed.
+End TM12.
+
+
+Module TM13.
+Definition tm := Eval compute in (TM_from_str "1LB0RC_1RC0LB_0RD1LB_0LA1RE_0RA1RF_1RC---").
+Notation "c -->* c'" := (c -[ tm ]->* c') (at level 40).
+Notation "c -->+ c'" := (c -[ tm ]->+ c') (at level 40).
+
+Notation h0 := ((A,<[1;0]),(B,[0;0])).
+Notation h1 := ((D,<[1;0;0;0]),(B,[0;0])).
+Notation h2 := ((C,<[1;1;0;1;1;1]),(B,[0;0])).
+Notation h3 := ((C,<[1;0;0;0;1;1;1]),(B,[0;0])).
+
+Definition f1 (w:seg)(h:head):option((list seg)*(list head)) :=
+List.find (fun '(x,y) => eqb x (h,w)) (
+((h0,[1;0;1;0]),([[1;0;1;0]],[h0;h0]))::
+((h0,[0;1;0]),([[1;1;0]],[]))::
+((h0,[1;1;0]),([[0;1;0]],[h0]))::
+((h1,[1;0;1;0]),([[1;0;1;0]],[h1;h0]))::
+((h1,[0;1;0]),([[0;1;0]],[h1]))::
+((h1,[1;1;0]),([],[h3]))::
+((h0,[1;0]),([],[h1]))::
+((h3,[1;0;1;0]),([[1;0;1;0];[1;1;0];[1;0]],[]))::
+((h3,[0;1;0]),([[1;0;1;0];[1;0;1;0]],[h0]))::
+((h3,[1;1;0]),([[1;0;1;0];[1;1;1;0]],[]))::
+((h0,[1;1;1;0]),([],[h2]))::
+((h2,[1;0;1;0]),([[0;1;0];[0;1;0];[1;0]],[]))::
+((h2,[1;1;0]),([[0;1;0];[0;1;1;0]],[]))::
+((h2,[0;1;0]),([[0;1;0];[0;0;1;0]],[h0]))::
+((h0,[0;1;1;0]),([[1;1;1;0]],[]))::
+((h0,[0;0;1;0]),([[1;0;1;0]],[]))::
+nil) &&& (fun '(x,y) => Some y).
+
+Definition f0 (w:seg)(h:head):option((list seg)*seg) :=
+List.find (fun '(x,y) => eqb x (h,w)) (
+((h0,[1]),([[0;1;0]],[1]))::
+((h1,[1]),([[1;0;1;0];[0;1;0]],[1]))::
+((h2,[1]),([[0;1;0];[0;1;0]],[]))::
+((h0,[]),([],[1]))::
+nil) &&& (fun '(x,y) => Some y).
+
+Definition f2 (w:seg)(h:head):option(N*N*head) :=
+List.find (fun '(x,y) => eqb x (h,w)) (
+((h0,[1;0;1;0]),(0%N,1%N,h0))::
+((h0,[0;1;0]),(1%N,0%N,h0))::
+((h0,[1;1;0]),(1%N,0%N,h0))::
+((h1,[0;1;0]),(0%N,0%N,h1))::
+nil) &&& (fun '(x,y) => Some y).
+
+Definition ws_init:(list seg)*seg := ([[1;0;1;0];[1;0;1;0];[1;0;1;0];[1;0;1;0];[1;0;1;0];[1;0;1;0];[1;0;1;0];[1;0;1;0];[1;0;1;0];[1;0;1;0];[1;0;1;0];[1;1;0];[0;1;0];[0;1;0];[0;1;0];[1;0;1;0];[1;1;0];[1;0;1;0];[1;1;0];[1;0;1;0];[1;1;0];[1;1;0];[1;1;0];[0;1;0];[0;1;0];[0;1;0];[0;1;0];[0;1;0]],[1]).
+
+Definition hs_step:(list head) := [h1]^^(387*4).
+
+Lemma nonhalt: ~halts tm c0.
+Proof.
+  eapply decide_nonhalt_spec with
+  (tm:=tm) (f2:=f2) (f1:=f1) (f0:=f0) (hs_step:=hs_step) (ws_init:=ws_init)
+  (lh:=0inf<*<[1;0]) (pp:=5%nat) (T:=N.to_nat (10^6)).
+  - intros.
+    unfold f2 in H.
+    apply find_spec in H.
+    gen w h a0 a1 h'.
+    apply f2_spec' with (T:=(10^3)).
+    time vm_compute; reflexivity.
+  - intros.
+    unfold f1 in H.
+    apply find_spec in H.
+    gen w h ws hs.
+    apply f1_spec' with (T:=(10^3)).
+    match goal with
+    | |- List.forallb ?f ?x = _ =>
+      pose (List.map f x) as v1;
+      vm_compute in v1
+    end.
+    time vm_compute; reflexivity.
+  - intros.
+    unfold f0 in H.
+    apply find_spec in H.
+    gen w h w'.
+    apply f0_spec' with (T:=(10^3)).
+    time vm_compute; reflexivity.
+  - reflexivity.
+  - intro X; inverts X.
+  - apply BoundedConfig.sideRLs_c_spec with (T:=10^4); reflexivity.
+  - esx.
+  - native_check_eq.
+Time Qed.
+End TM13.
+
