verify/SOMDCv6.v
@@ -1,0 +1,1626 @@
+From BusyCoq Require Import Individual62 Longitudinal DivModCases.
+Require Import ZifyNat Lia.
+Require Import ZArith.
+Require Import String.
+Require Import List.
+
+
+Ltac esc :=
+  (apply BoundedConfig.segRLs_c_spec with (T:=10^3); reflexivity) ||
+  (apply BoundedConfig.sideRLs_c_spec with (T:=10^3); reflexivity) ||
+  (eapply sideRLs_c_spec with (T:=10^6); [vm_compute; reflexivity | st; reflexivity]).
+
+Ltac ec := econstructor.
+
+Ltac am a a' k b b' :=
+  applys_eq (segRLs_addmul_v2 a a' k b b'); unfold DH0; flia; esc.
+
+Module TM1.
+Definition tm := Eval compute in (TM_from_str "1LB1RE_0LC0RC_1RD0LE_0RA0LB_1RF0LD_0RB---").
+Notation "c -->* c'" := (c -[ tm ]->* c') (at level 40).
+Notation "c -->+ c'" := (c -[ tm ]->+ c') (at level 40).
+
+Notation ld := [1;0;0;1;0;0].
+Notation d0 := [0;0;0;0].
+Notation d1 := [1;0;0;0].
+Notation hR := (A,[0]).
+Notation hL := (C,[0]).
+Notation h := [(hR,hL)].
+
+Inductive RD := LD|D0|D1.
+Inductive H := h100|h000|h0.
+
+Fixpoint toRC ls :=
+match ls with
+| [] => 0inf
+| LD::ls => ld*>toRC ls
+| D0::ls => d0*>toRC ls
+| D1::ls => d1*>toRC ls
+end.
+
+Definition toH x :=
+match x with
+| h100 => [1;0;0]
+| h000 => [0;0;0]
+| h0 => [0]
+end.
+
+Inductive RIncs: H->nat->(list RD)->(list RD)->Prop :=
+| RIncs_100_ld k r r':
+  RIncs h100 (k*2) r r' ->
+  RIncs h100 k (LD::r) (LD::r')
+| RIncs_000_ld k r r':
+  RIncs h100 (k*2) r r' ->
+  RIncs h000 (1+k) (LD::r) (LD::r')
+| RIncs_0_ld_0 k r r':
+  RIncs h100 k r r' ->
+  RIncs h0 (2+k*2) (LD::r) (D0::r')
+| RIncs_0_ld_1 k r r':
+  RIncs h100 k r r' ->
+  RIncs h0 (3+k*2) (LD::r) (D1::r')
+
+| RIncs_100_d0_0 k r r':
+  RIncs h000 k r r' ->
+  RIncs h100 (k*2) (D0::r) (D1::r')
+| RIncs_100_d0_1 k r r':
+  RIncs h000 (1+k) r r' ->
+  RIncs h100 (1+k*2) (D0::r) (D0::r')
+| RIncs_000_d0_0 k r r':
+  RIncs h000 k r r' ->
+  RIncs h000 (k*2) (D0::r) (D0::r')
+| RIncs_000_d0_1 k r r':
+  RIncs h000 k r r' ->
+  RIncs h000 (1+k*2) (D0::r) (D1::r')
+| RIncs_0_d0_0 k r r':
+  RIncs h0 k r r' ->
+  RIncs h0 (k*2) (D0::r) (D0::r')
+| RIncs_0_d0_1 k r r':
+  RIncs h0 k r r' ->
+  RIncs h0 (1+k*2) (D0::r) (D1::r')
+
+| RIncs_100_d1 k r r':
+  RIncs h0 (k*2) r r' ->
+  RIncs h100 k (D1::r) (LD::r')
+| RIncs_000_d1 k r r':
+  RIncs h0 (k*2) r r' ->
+  RIncs h000 (1+k) (D1::r) (LD::r')
+| RIncs_0_d1_0 k r r':
+  RIncs h0 k r r' ->
+  RIncs h0 (2+k*2) (D1::r) (D0::r')
+| RIncs_0_d1_1 k r r':
+  RIncs h0 k r r' ->
+  RIncs h0 (3+k*2) (D1::r) (D1::r')
+
+| RIncs_100_rh:
+  RIncs h100 0 [] [D1]
+| RIncs_100_rh':
+  RIncs h100 1 [] [D0;D1]
+| RIncs_000_rh:
+  RIncs h000 0 [] []
+| RIncs_0_rh:
+  RIncs h0 0 [] []
+
+| RIncs_100_rh_0 k r':
+  RIncs h000 (1+k) [] r' ->
+  RIncs h100 (2+k*2) [] (D1::r')
+| RIncs_100_rh_1 k r':
+  RIncs h000 (2+k) [] r' ->
+  RIncs h100 (3+k*2) [] (D0::r')
+| RIncs_000_rh_0 k r':
+  RIncs h000 (1+k) [] r' ->
+  RIncs h000 (2+k*2) [] (D0::r')
+| RIncs_000_rh_1 k r':
+  RIncs h000 k [] r' ->
+  RIncs h000 (1+k*2) [] (D1::r')
+| RIncs_0_rh_0 k r':
+  RIncs h0 (1+k) [] r' ->
+  RIncs h0 (2+k*2) [] (D0::r')
+| RIncs_0_rh_1 k r':
+  RIncs h0 k [] r' ->
+  RIncs h0 (1+k*2) [] (D1::r')
+.
+
+Ltac cat6 :=
+  eapply @segRLs_sideRLs_concat with (w1:=[_;_;_;_;_;_]) (w2:=[_;_;_;_;_;_]); [|eauto 1].
+
+Ltac cat4 :=
+  eapply @segRLs_sideRLs_concat with (w1:=[_;_;_;_]) (w2:=[_;_;_;_]); [|eauto 1].
+
+Ltac cat4' :=
+  do 4 rewrite const_unfold; cat4.
+
+Open Scope nat.
+
+Lemma RIncs_spec tp k r r':
+  RIncs tp k r r' ->
+  sideRLs tm (h^^k) (toH tp*>toRC r) (toRC r').
+Proof.
+  intro H.
+  induction H; intros; cbn[toH toRC] in *.
+  - cat6. am 1 2 k 0 0.
+  - cat6. am 1 2 k 1 0.
+  - cat4. am 2 1 k 2 0.
+  - cat4. am 2 1 k 3 0.
+
+  - cat4. am 2 1 k 0 0.
+  - cat4. am 2 1 k 1 1.
+  - cat4. am 2 1 k 0 0.
+  - cat4. am 2 1 k 1 0.
+  - cat4. am 2 1 k 0 0.
+  - cat4. am 2 1 k 1 0.
+
+  - cat6. am 1 2 k 0 0.
+  - cat6. am 1 2 k 1 0.
+  - cat4. am 2 1 k 2 0.
+  - cat4. am 2 1 k 3 0.
+
+  - esc.
+  - esc.
+  - esc.
+  - esc.
+  - cat4'. am 2 1 (1+k) 0 0.
+  - cat4'. am 2 1 (1+k) 1 1.
+  - cat4'. am 2 1 (1+k) 0 0.
+  - cat4'. am 2 1 k 1 0.
+  - cat4'. am 2 1 (1+k) 0 0.
+  - cat4'. am 2 1 k 1 0.
+Qed.
+
+
+Lemma RIncs_nxt_0 k:
+  exists r, RIncs h0 k [] r.
+Proof.
+  induction k using lt_wf_ind.
+  destruct k.
+  + ec. ec.
+  + destruct (mod2 k); subst.
+    * epose proof (H0 _ _) as [r I].
+      ec. ec. apply I.
+    * epose proof (H0 _ _) as [r I].
+      ec. ec. apply I.
+  Unshelve. all: lia.
+Qed.
+
+Lemma RIncs_nxt_000 k:
+  exists r, RIncs h000 k [] r.
+Proof.
+  induction k using lt_wf_ind.
+  destruct k.
+  + ec. ec.
+  + destruct (mod2 k); subst.
+    * epose proof (H0 _ _) as [r I].
+      ec. ec. apply I.
+    * epose proof (H0 _ _) as [r I].
+      ec. ec. apply I.
+  Unshelve. all: lia.
+Qed.
+
+Lemma RIncs_nxt_100 k:
+  exists r, RIncs h100 k [] r.
+Proof.
+  destruct k as [|[|k]].
+  - ec. ec.
+  - ec. ec.
+  - destruct (mod2 k); subst.
+    * epose proof (RIncs_nxt_000 _) as [r I].
+      ec. ec. apply I.
+    * epose proof (RIncs_nxt_000 _) as [r I].
+      ec. ec. apply I.
+Qed.
+
+Ltac solve_v2 :=
+  (epose proof (RIncs_nxt_0 _) as [r I]; repeat ec; apply I) ||
+  (epose proof (RIncs_nxt_000 _) as [r I]; repeat ec; apply I) ||
+  (epose proof (RIncs_nxt_100 _) as [r I]; repeat ec; apply I).
+
+Ltac solve_v1 H tp'0 k'0 H' :=
+  eapply H with (tp':=tp'0) (k':=k'0) in H';
+  try lia;
+  try (
+  destruct H' as [r'' I1];
+  repeat ec; try apply I1).
+
+Lemma RIncs_nxt tp k r r' tp' k':
+  RIncs tp k r r' ->
+  match tp,tp' with
+  | h100,h100 => k<=k'
+  | h100,h000 => 1+k<=k'
+  | h000,h000 => k<=k'
+  | h000,h0 => k*4<=k'
+  | h100,h0 => 4+k*4<=k'
+  | h0,h100 => k<=k'
+  | h0,h000 => k<=k'
+  | h0,h0 => k*4<=k'
+  | _,_ => False
+  end ->
+  exists r'',
+  RIncs tp' k' r' r''.
+Proof.
+  gen tp k r' tp' k'.
+  induction r; intros.
+  {
+    gen tp r' tp' k'.
+    induction k using lt_wf_ind.
+    intros.
+    inverts H1; destruct tp'.
+    all: try lia.
+    - solve_v2.
+    - destruct (sub k' 1); [subst|lia].
+      solve_v2.
+    - destruct (sub k' 2); [subst|lia].
+      destruct (mod2 c); subst.
+      + solve_v2.
+      + solve_v2.
+    - destruct (mod2 k'); subst.
+      + destruct (sub a 1); [subst|lia].
+        solve_v2.
+      + solve_v2.
+    - destruct (mod2 k'); subst.
+      + destruct (sub a 1); [subst|lia].
+        solve_v2.
+      + destruct (sub a 1); [subst|lia].
+        solve_v2.
+    - destruct (mod2 k'); subst.
+      + destruct (sub a 2); [subst|lia].
+        destruct (mod2 c); subst.
+        * solve_v2.
+        * solve_v2.
+      + destruct (sub a 2); [subst|lia].
+        destruct (mod2 c); subst.
+        * solve_v2.
+        * solve_v2.
+    - solve_v2.
+    - solve_v2.
+    - solve_v2.
+    - solve_v2.
+    - solve_v2.
+    - solve_v1 H0 h0 (k'*2) H3.
+    - destruct (sub k' 1); [subst|lia].
+      solve_v1 H0 h0 (c*2) H3.
+    - destruct (sub k' 2); [subst|lia].
+      destruct (mod2 c); subst.
+      + solve_v1 H0 h0 a H3.
+      + solve_v1 H0 h0 a H3.
+    - destruct (mod2 k'); subst.
+      + solve_v1 H0 h000 a H3.
+      + solve_v1 H0 h000 (1+a) H3.
+    - destruct (mod2 k'); subst.
+      + solve_v1 H0 h000 a H3.
+      + solve_v1 H0 h000 a H3.
+    - destruct (mod2 k'); subst.
+      + solve_v1 H0 h0 a H3.
+      + solve_v1 H0 h0 a H3.
+    - destruct (mod2 k'); subst.
+      + solve_v1 H0 h000 a H3.
+      + solve_v1 H0 h000 a H3.
+    - destruct (mod2 k'); subst.
+      + solve_v1 H0 h0 a H3.
+      + solve_v1 H0 h0 a H3.
+    - destruct (sub k' 1); [subst|lia].
+      solve_v1 H0 h0 (c*2) H3.
+    - destruct (sub k' 2); [subst|lia].
+      destruct (mod2 c); subst.
+      + solve_v1 H0 h0 a H3.
+      + solve_v1 H0 h0 a H3.
+    - destruct (mod2 k'); subst.
+      + solve_v1 H0 h000 a H3.
+      + solve_v1 H0 h000 (1+a) H3.
+    - destruct (mod2 k'); subst.
+      + solve_v1 H0 h000 a H3.
+      + solve_v1 H0 h000 a H3.
+    - destruct (mod2 k'); subst.
+      + solve_v1 H0 h0 a H3.
+      + solve_v1 H0 h0 a H3.
+    - solve_v1 H0 h0 (k'*2) H3.
+    - destruct (sub k' 1); [subst|lia].
+      solve_v1 H0 h0 (c*2) H3.
+    - destruct (sub k' 2); [subst|lia].
+      destruct (mod2 c); subst.
+      + solve_v1 H0 h0 a H3.
+      + solve_v1 H0 h0 a H3.
+  }
+  {
+    inverts H0; destruct tp'.
+    all: try lia.
+    - solve_v1 IHr h100 (k'*2) H7.
+    - destruct (sub k' 1); [subst|lia].
+      solve_v1 IHr h100 (c*2) H7.
+    - destruct (sub k' 2); [subst|lia].
+      destruct (mod2 c); subst.
+      + solve_v1 IHr h100 a H7.
+      + solve_v1 IHr h100 a H7.
+    - destruct (sub k' 1); [subst|lia].
+      solve_v1 IHr h100 (c*2) H7.
+    - destruct (sub k' 2); [subst|lia].
+      destruct (mod2 c); subst.
+      + solve_v1 IHr h100 a H7.
+      + solve_v1 IHr h100 a H7.
+    - destruct (mod2 k'); subst.
+      + solve_v1 IHr h000 a H7.
+      + solve_v1 IHr h000 (1+a) H7.
+    - destruct (mod2 k'); subst.
+      + solve_v1 IHr h000 a H7.
+      + solve_v1 IHr h000 a H7.
+    - destruct (mod2 k'); subst.
+      + solve_v1 IHr h0 a H7.
+      + solve_v1 IHr h0 a H7.
+    - solve_v1 IHr h0 (k'*2) H7.
+    - destruct (sub k' 1); [subst|lia].
+      solve_v1 IHr h0 (c*2) H7.
+    - destruct (sub k' 2); [subst|lia].
+      destruct (mod2 c); subst.
+      + solve_v1 IHr h0 a H7.
+      + solve_v1 IHr h0 a H7.
+    - solve_v1 IHr h0 (k'*2) H7.
+    - destruct (sub k' 1); [subst|lia].
+      solve_v1 IHr h0 (c*2) H7.
+    - destruct (sub k' 2); [subst|lia].
+      destruct (mod2 c); subst.
+      + solve_v1 IHr h0 a H7.
+      + solve_v1 IHr h0 a H7.
+    - destruct (mod2 k'); subst.
+      + solve_v1 IHr h000 a H7.
+      + solve_v1 IHr h000 (1+a) H7.
+    - destruct (mod2 k'); subst.
+      + solve_v1 IHr h000 a H7.
+      + solve_v1 IHr h000 a H7.
+    - destruct (mod2 k'); subst.
+      + solve_v1 IHr h0 a H7.
+      + solve_v1 IHr h0 a H7.
+    - destruct (mod2 k'); subst.
+      + solve_v1 IHr h000 a H7.
+      + solve_v1 IHr h000 a H7.
+    - destruct (mod2 k'); subst.
+      + solve_v1 IHr h0 a H7.
+      + solve_v1 IHr h0 a H7.
+    - destruct (sub k' 1); [subst|lia].
+      solve_v1 IHr h0 (c*2) H7.
+    - destruct (sub k' 2); [subst|lia].
+      destruct (mod2 c); subst.
+      + solve_v1 IHr h0 a H7.
+      + solve_v1 IHr h0 a H7.
+    - destruct (mod2 k'); subst.
+      + solve_v1 IHr h000 a H7.
+      + solve_v1 IHr h000 (1+a) H7.
+    - destruct (mod2 k'); subst.
+      + solve_v1 IHr h000 a H7.
+      + solve_v1 IHr h000 a H7.
+    - destruct (mod2 k'); subst.
+      + solve_v1 IHr h0 a H7.
+      + solve_v1 IHr h0 a H7.
+    - solve_v1 IHr h0 (k'*2) H7.
+    - destruct (sub k' 1); [subst|lia].
+      solve_v1 IHr h0 (c*2) H7.
+    - destruct (sub k' 2); [subst|lia].
+      destruct (mod2 c); subst.
+      + solve_v1 IHr h0 a H7.
+      + solve_v1 IHr h0 a H7.
+    - solve_v1 IHr h100 (k'*2) H7.
+    - destruct (sub k' 1); [subst|lia].
+      solve_v1 IHr h100 (c*2) H7.
+    - destruct (sub k' 2); [subst|lia].
+      destruct (mod2 c); subst.
+      + solve_v1 IHr h100 a H7.
+      + solve_v1 IHr h100 a H7.
+    - destruct (sub k' 1); [subst|lia].
+      solve_v1 IHr h100 (c*2) H7.
+    - destruct (sub k' 2); [subst|lia].
+      destruct (mod2 c); subst.
+      + solve_v1 IHr h100 a H7.
+      + solve_v1 IHr h100 a H7.
+    - destruct (mod2 k'); subst.
+      + solve_v1 IHr h000 a H7.
+      + solve_v1 IHr h000 (1+a) H7.
+    - destruct (mod2 k'); subst.
+      + solve_v1 IHr h000 a H7.
+      + solve_v1 IHr h000 a H7.
+    - destruct (mod2 k'); subst.
+      + solve_v1 IHr h0 a H7.
+      + solve_v1 IHr h0 a H7.
+    - solve_v1 IHr h0 (k'*2) H7.
+    - destruct (sub k' 1); [subst|lia].
+      solve_v1 IHr h0 (c*2) H7.
+    - destruct (sub k' 2); [subst|lia].
+      destruct (mod2 c); subst.
+      + solve_v1 IHr h0 a H7.
+      + solve_v1 IHr h0 a H7.
+  }
+Qed.
+
+Open Scope sym.
+
+Notation lh := (0inf<*<[1]).
+Notation lh' := (0inf<*<[1;1]).
+
+Lemma LRst:
+  sideRLs (flip tm) [(hL,hR)] lh lh'.
+Proof.
+  esc.
+Qed.
+
+Definition S' r :=
+  lh {{{ (hR,R) }}} toH h100 *> toRC r.
+
+Lemma BigStep r r':
+  RIncs h100 2 r r' ->
+  S' r -->+ S' r'.
+Proof.
+  intros H.
+  apply RIncs_spec in H.
+  follow10 (sideRLs_concat LRst H).
+  es.
+Qed.
+
+Lemma nonhalt: ~halts tm c0.
+Proof.
+  eapply multistep_nonhalt with (c':=S' [LD;D0;D1]).
+  1: esx.
+  eapply progress_nonhalt_cond with (P:=fun r => exists r', RIncs h100 2 r r').
+  2: {
+    do 5 ec.
+    change (1+0) with (1+0*2).
+    do 2 ec.
+  }
+  intros r [r' I1].
+  pose proof I1 as I2.
+  eapply RIncs_nxt with (tp':=h100) (k':=2) in I2.
+  2: lia.
+  exists r'; split.
+  - apply BigStep,I1.
+  - apply I2.
+Qed.
+
+End TM1.
+
+
+Module TM2.
+Definition tm := Eval compute in (TM_from_str "1LB1RE_0LC0RF_1RD0LE_0RA0LB_1RF0LD_0RB---").
+Notation "c -->* c'" := (c -[ tm ]->* c') (at level 40).
+Notation "c -->+ c'" := (c -[ tm ]->+ c') (at level 40).
+
+Notation ld := [1;0;0;1;0;0].
+Notation d0 := [0;0;0;0].
+Notation d1 := [1;0;0;0].
+Notation hR := (A,[0]).
+Notation hL := (C,[0]).
+Notation h := [(hR,hL)].
+
+Inductive RD := LD|D0|D1.
+Inductive H := h100|h000|h0.
+
+Fixpoint toRC ls :=
+match ls with
+| [] => 0inf
+| LD::ls => ld*>toRC ls
+| D0::ls => d0*>toRC ls
+| D1::ls => d1*>toRC ls
+end.
+
+Definition toH x :=
+match x with
+| h100 => [1;0;0]
+| h000 => [0;0;0]
+| h0 => [0]
+end.
+
+Inductive RIncs: H->nat->(list RD)->(list RD)->Prop :=
+| RIncs_100_ld k r r':
+  RIncs h100 (k*2) r r' ->
+  RIncs h100 k (LD::r) (LD::r')
+| RIncs_000_ld k r r':
+  RIncs h100 (k*2) r r' ->
+  RIncs h000 (1+k) (LD::r) (LD::r')
+| RIncs_0_ld_0 k r r':
+  RIncs h100 k r r' ->
+  RIncs h0 (2+k*2) (LD::r) (D0::r')
+| RIncs_0_ld_1 k r r':
+  RIncs h100 k r r' ->
+  RIncs h0 (3+k*2) (LD::r) (D1::r')
+
+| RIncs_100_d0_0 k r r':
+  RIncs h000 k r r' ->
+  RIncs h100 (k*2) (D0::r) (D1::r')
+| RIncs_100_d0_1 k r r':
+  RIncs h000 (1+k) r r' ->
+  RIncs h100 (1+k*2) (D0::r) (D0::r')
+| RIncs_000_d0_0 k r r':
+  RIncs h000 k r r' ->
+  RIncs h000 (k*2) (D0::r) (D0::r')
+| RIncs_000_d0_1 k r r':
+  RIncs h000 k r r' ->
+  RIncs h000 (1+k*2) (D0::r) (D1::r')
+| RIncs_0_d0_0 k r r':
+  RIncs h0 k r r' ->
+  RIncs h0 (k*2) (D0::r) (D0::r')
+| RIncs_0_d0_1 k r r':
+  RIncs h0 k r r' ->
+  RIncs h0 (1+k*2) (D0::r) (D1::r')
+
+| RIncs_100_d1 k r r':
+  RIncs h0 (k*2) r r' ->
+  RIncs h100 k (D1::r) (LD::r')
+| RIncs_000_d1 k r r':
+  RIncs h0 (k*2) r r' ->
+  RIncs h000 (1+k) (D1::r) (LD::r')
+| RIncs_0_d1_0 k r r':
+  RIncs h0 k r r' ->
+  RIncs h0 (2+k*2) (D1::r) (D0::r')
+| RIncs_0_d1_1 k r r':
+  RIncs h0 k r r' ->
+  RIncs h0 (3+k*2) (D1::r) (D1::r')
+
+| RIncs_100_rh:
+  RIncs h100 0 [] [D1]
+| RIncs_100_rh':
+  RIncs h100 1 [] [D0;D1]
+| RIncs_000_rh:
+  RIncs h000 0 [] []
+| RIncs_0_rh:
+  RIncs h0 0 [] []
+
+| RIncs_100_rh_0 k r':
+  RIncs h000 (1+k) [] r' ->
+  RIncs h100 (2+k*2) [] (D1::r')
+| RIncs_100_rh_1 k r':
+  RIncs h000 (2+k) [] r' ->
+  RIncs h100 (3+k*2) [] (D0::r')
+| RIncs_000_rh_0 k r':
+  RIncs h000 (1+k) [] r' ->
+  RIncs h000 (2+k*2) [] (D0::r')
+| RIncs_000_rh_1 k r':
+  RIncs h000 k [] r' ->
+  RIncs h000 (1+k*2) [] (D1::r')
+| RIncs_0_rh_0 k r':
+  RIncs h0 (1+k) [] r' ->
+  RIncs h0 (2+k*2) [] (D0::r')
+| RIncs_0_rh_1 k r':
+  RIncs h0 k [] r' ->
+  RIncs h0 (1+k*2) [] (D1::r')
+.
+
+Ltac cat6 :=
+  eapply @segRLs_sideRLs_concat with (w1:=[_;_;_;_;_;_]) (w2:=[_;_;_;_;_;_]); [|eauto 1].
+
+Ltac cat4 :=
+  eapply @segRLs_sideRLs_concat with (w1:=[_;_;_;_]) (w2:=[_;_;_;_]); [|eauto 1].
+
+Ltac cat4' :=
+  do 4 rewrite const_unfold; cat4.
+
+Open Scope nat.
+
+Lemma RIncs_spec tp k r r':
+  RIncs tp k r r' ->
+  sideRLs tm (h^^k) (toH tp*>toRC r) (toRC r').
+Proof.
+  intro H.
+  induction H; intros; cbn[toH toRC] in *.
+  - cat6. am 1 2 k 0 0.
+  - cat6. am 1 2 k 1 0.
+  - cat4. am 2 1 k 2 0.
+  - cat4. am 2 1 k 3 0.
+
+  - cat4. am 2 1 k 0 0.
+  - cat4. am 2 1 k 1 1.
+  - cat4. am 2 1 k 0 0.
+  - cat4. am 2 1 k 1 0.
+  - cat4. am 2 1 k 0 0.
+  - cat4. am 2 1 k 1 0.
+
+  - cat6. am 1 2 k 0 0.
+  - cat6. am 1 2 k 1 0.
+  - cat4. am 2 1 k 2 0.
+  - cat4. am 2 1 k 3 0.
+
+  - esc.
+  - esc.
+  - esc.
+  - esc.
+  - cat4'. am 2 1 (1+k) 0 0.
+  - cat4'. am 2 1 (1+k) 1 1.
+  - cat4'. am 2 1 (1+k) 0 0.
+  - cat4'. am 2 1 k 1 0.
+  - cat4'. am 2 1 (1+k) 0 0.
+  - cat4'. am 2 1 k 1 0.
+Qed.
+
+
+Lemma RIncs_nxt_0 k:
+  exists r, RIncs h0 k [] r.
+Proof.
+  induction k using lt_wf_ind.
+  destruct k.
+  + ec. ec.
+  + destruct (mod2 k); subst.
+    * epose proof (H0 _ _) as [r I].
+      ec. ec. apply I.
+    * epose proof (H0 _ _) as [r I].
+      ec. ec. apply I.
+  Unshelve. all: lia.
+Qed.
+
+Lemma RIncs_nxt_000 k:
+  exists r, RIncs h000 k [] r.
+Proof.
+  induction k using lt_wf_ind.
+  destruct k.
+  + ec. ec.
+  + destruct (mod2 k); subst.
+    * epose proof (H0 _ _) as [r I].
+      ec. ec. apply I.
+    * epose proof (H0 _ _) as [r I].
+      ec. ec. apply I.
+  Unshelve. all: lia.
+Qed.
+
+Lemma RIncs_nxt_100 k:
+  exists r, RIncs h100 k [] r.
+Proof.
+  destruct k as [|[|k]].
+  - ec. ec.
+  - ec. ec.
+  - destruct (mod2 k); subst.
+    * epose proof (RIncs_nxt_000 _) as [r I].
+      ec. ec. apply I.
+    * epose proof (RIncs_nxt_000 _) as [r I].
+      ec. ec. apply I.
+Qed.
+
+Ltac solve_v2 :=
+  (epose proof (RIncs_nxt_0 _) as [r I]; repeat ec; apply I) ||
+  (epose proof (RIncs_nxt_000 _) as [r I]; repeat ec; apply I) ||
+  (epose proof (RIncs_nxt_100 _) as [r I]; repeat ec; apply I).
+
+Ltac solve_v1 H tp'0 k'0 H' :=
+  eapply H with (tp':=tp'0) (k':=k'0) in H';
+  try lia;
+  try (
+  destruct H' as [r'' I1];
+  repeat ec; try apply I1).
+
+Lemma RIncs_nxt tp k r r' tp' k':
+  RIncs tp k r r' ->
+  match tp,tp' with
+  | h100,h100 => k<=k'
+  | h100,h000 => 1+k<=k'
+  | h000,h000 => k<=k'
+  | h000,h0 => k*4<=k'
+  | h100,h0 => 4+k*4<=k'
+  | h0,h100 => k<=k'
+  | h0,h000 => k<=k'
+  | h0,h0 => k*4<=k'
+  | _,_ => False
+  end ->
+  exists r'',
+  RIncs tp' k' r' r''.
+Proof.
+  gen tp k r' tp' k'.
+  induction r; intros.
+  {
+    gen tp r' tp' k'.
+    induction k using lt_wf_ind.
+    intros.
+    inverts H1; destruct tp'.
+    all: try lia.
+    - solve_v2.
+    - destruct (sub k' 1); [subst|lia].
+      solve_v2.
+    - destruct (sub k' 2); [subst|lia].
+      destruct (mod2 c); subst.
+      + solve_v2.
+      + solve_v2.
+    - destruct (mod2 k'); subst.
+      + destruct (sub a 1); [subst|lia].
+        solve_v2.
+      + solve_v2.
+    - destruct (mod2 k'); subst.
+      + destruct (sub a 1); [subst|lia].
+        solve_v2.
+      + destruct (sub a 1); [subst|lia].
+        solve_v2.
+    - destruct (mod2 k'); subst.
+      + destruct (sub a 2); [subst|lia].
+        destruct (mod2 c); subst.
+        * solve_v2.
+        * solve_v2.
+      + destruct (sub a 2); [subst|lia].
+        destruct (mod2 c); subst.
+        * solve_v2.
+        * solve_v2.
+    - solve_v2.
+    - solve_v2.
+    - solve_v2.
+    - solve_v2.
+    - solve_v2.
+    - solve_v1 H0 h0 (k'*2) H3.
+    - destruct (sub k' 1); [subst|lia].
+      solve_v1 H0 h0 (c*2) H3.
+    - destruct (sub k' 2); [subst|lia].
+      destruct (mod2 c); subst.
+      + solve_v1 H0 h0 a H3.
+      + solve_v1 H0 h0 a H3.
+    - destruct (mod2 k'); subst.
+      + solve_v1 H0 h000 a H3.
+      + solve_v1 H0 h000 (1+a) H3.
+    - destruct (mod2 k'); subst.
+      + solve_v1 H0 h000 a H3.
+      + solve_v1 H0 h000 a H3.
+    - destruct (mod2 k'); subst.
+      + solve_v1 H0 h0 a H3.
+      + solve_v1 H0 h0 a H3.
+    - destruct (mod2 k'); subst.
+      + solve_v1 H0 h000 a H3.
+      + solve_v1 H0 h000 a H3.
+    - destruct (mod2 k'); subst.
+      + solve_v1 H0 h0 a H3.
+      + solve_v1 H0 h0 a H3.
+    - destruct (sub k' 1); [subst|lia].
+      solve_v1 H0 h0 (c*2) H3.
+    - destruct (sub k' 2); [subst|lia].
+      destruct (mod2 c); subst.
+      + solve_v1 H0 h0 a H3.
+      + solve_v1 H0 h0 a H3.
+    - destruct (mod2 k'); subst.
+      + solve_v1 H0 h000 a H3.
+      + solve_v1 H0 h000 (1+a) H3.
+    - destruct (mod2 k'); subst.
+      + solve_v1 H0 h000 a H3.
+      + solve_v1 H0 h000 a H3.
+    - destruct (mod2 k'); subst.
+      + solve_v1 H0 h0 a H3.
+      + solve_v1 H0 h0 a H3.
+    - solve_v1 H0 h0 (k'*2) H3.
+    - destruct (sub k' 1); [subst|lia].
+      solve_v1 H0 h0 (c*2) H3.
+    - destruct (sub k' 2); [subst|lia].
+      destruct (mod2 c); subst.
+      + solve_v1 H0 h0 a H3.
+      + solve_v1 H0 h0 a H3.
+  }
+  {
+    inverts H0; destruct tp'.
+    all: try lia.
+    - solve_v1 IHr h100 (k'*2) H7.
+    - destruct (sub k' 1); [subst|lia].
+      solve_v1 IHr h100 (c*2) H7.
+    - destruct (sub k' 2); [subst|lia].
+      destruct (mod2 c); subst.
+      + solve_v1 IHr h100 a H7.
+      + solve_v1 IHr h100 a H7.
+    - destruct (sub k' 1); [subst|lia].
+      solve_v1 IHr h100 (c*2) H7.
+    - destruct (sub k' 2); [subst|lia].
+      destruct (mod2 c); subst.
+      + solve_v1 IHr h100 a H7.
+      + solve_v1 IHr h100 a H7.
+    - destruct (mod2 k'); subst.
+      + solve_v1 IHr h000 a H7.
+      + solve_v1 IHr h000 (1+a) H7.
+    - destruct (mod2 k'); subst.
+      + solve_v1 IHr h000 a H7.
+      + solve_v1 IHr h000 a H7.
+    - destruct (mod2 k'); subst.
+      + solve_v1 IHr h0 a H7.
+      + solve_v1 IHr h0 a H7.
+    - solve_v1 IHr h0 (k'*2) H7.
+    - destruct (sub k' 1); [subst|lia].
+      solve_v1 IHr h0 (c*2) H7.
+    - destruct (sub k' 2); [subst|lia].
+      destruct (mod2 c); subst.
+      + solve_v1 IHr h0 a H7.
+      + solve_v1 IHr h0 a H7.
+    - solve_v1 IHr h0 (k'*2) H7.
+    - destruct (sub k' 1); [subst|lia].
+      solve_v1 IHr h0 (c*2) H7.
+    - destruct (sub k' 2); [subst|lia].
+      destruct (mod2 c); subst.
+      + solve_v1 IHr h0 a H7.
+      + solve_v1 IHr h0 a H7.
+    - destruct (mod2 k'); subst.
+      + solve_v1 IHr h000 a H7.
+      + solve_v1 IHr h000 (1+a) H7.
+    - destruct (mod2 k'); subst.
+      + solve_v1 IHr h000 a H7.
+      + solve_v1 IHr h000 a H7.
+    - destruct (mod2 k'); subst.
+      + solve_v1 IHr h0 a H7.
+      + solve_v1 IHr h0 a H7.
+    - destruct (mod2 k'); subst.
+      + solve_v1 IHr h000 a H7.
+      + solve_v1 IHr h000 a H7.
+    - destruct (mod2 k'); subst.
+      + solve_v1 IHr h0 a H7.
+      + solve_v1 IHr h0 a H7.
+    - destruct (sub k' 1); [subst|lia].
+      solve_v1 IHr h0 (c*2) H7.
+    - destruct (sub k' 2); [subst|lia].
+      destruct (mod2 c); subst.
+      + solve_v1 IHr h0 a H7.
+      + solve_v1 IHr h0 a H7.
+    - destruct (mod2 k'); subst.
+      + solve_v1 IHr h000 a H7.
+      + solve_v1 IHr h000 (1+a) H7.
+    - destruct (mod2 k'); subst.
+      + solve_v1 IHr h000 a H7.
+      + solve_v1 IHr h000 a H7.
+    - destruct (mod2 k'); subst.
+      + solve_v1 IHr h0 a H7.
+      + solve_v1 IHr h0 a H7.
+    - solve_v1 IHr h0 (k'*2) H7.
+    - destruct (sub k' 1); [subst|lia].
+      solve_v1 IHr h0 (c*2) H7.
+    - destruct (sub k' 2); [subst|lia].
+      destruct (mod2 c); subst.
+      + solve_v1 IHr h0 a H7.
+      + solve_v1 IHr h0 a H7.
+    - solve_v1 IHr h100 (k'*2) H7.
+    - destruct (sub k' 1); [subst|lia].
+      solve_v1 IHr h100 (c*2) H7.
+    - destruct (sub k' 2); [subst|lia].
+      destruct (mod2 c); subst.
+      + solve_v1 IHr h100 a H7.
+      + solve_v1 IHr h100 a H7.
+    - destruct (sub k' 1); [subst|lia].
+      solve_v1 IHr h100 (c*2) H7.
+    - destruct (sub k' 2); [subst|lia].
+      destruct (mod2 c); subst.
+      + solve_v1 IHr h100 a H7.
+      + solve_v1 IHr h100 a H7.
+    - destruct (mod2 k'); subst.
+      + solve_v1 IHr h000 a H7.
+      + solve_v1 IHr h000 (1+a) H7.
+    - destruct (mod2 k'); subst.
+      + solve_v1 IHr h000 a H7.
+      + solve_v1 IHr h000 a H7.
+    - destruct (mod2 k'); subst.
+      + solve_v1 IHr h0 a H7.
+      + solve_v1 IHr h0 a H7.
+    - solve_v1 IHr h0 (k'*2) H7.
+    - destruct (sub k' 1); [subst|lia].
+      solve_v1 IHr h0 (c*2) H7.
+    - destruct (sub k' 2); [subst|lia].
+      destruct (mod2 c); subst.
+      + solve_v1 IHr h0 a H7.
+      + solve_v1 IHr h0 a H7.
+  }
+Qed.
+
+Open Scope sym.
+
+Notation lh := (0inf<*<[1]).
+Notation lh' := (0inf<*<[1;1]).
+
+Lemma LRst:
+  sideRLs (flip tm) [(hL,hR)] lh lh'.
+Proof.
+  esc.
+Qed.
+
+Definition S' r :=
+  lh {{{ (hR,R) }}} toH h100 *> toRC r.
+
+Lemma BigStep r r':
+  RIncs h100 2 r r' ->
+  S' r -->+ S' r'.
+Proof.
+  intros H.
+  apply RIncs_spec in H.
+  follow10 (sideRLs_concat LRst H).
+  es.
+Qed.
+
+Lemma nonhalt: ~halts tm c0.
+Proof.
+  eapply multistep_nonhalt with (c':=S' [LD;D0;D1]).
+  1: esx.
+  eapply progress_nonhalt_cond with (P:=fun r => exists r', RIncs h100 2 r r').
+  2: {
+    do 5 ec.
+    change (1+0) with (1+0*2).
+    do 2 ec.
+  }
+  intros r [r' I1].
+  pose proof I1 as I2.
+  eapply RIncs_nxt with (tp':=h100) (k':=2) in I2.
+  2: lia.
+  exists r'; split.
+  - apply BigStep,I1.
+  - apply I2.
+Qed.
+
+End TM2.
+
+
+Module TM3.
+Definition tm := Eval compute in (TM_from_str "1RB1RE_0LC1LB_1RD1LB_1RA0LB_0RD0RF_---0RA").
+Notation "c -->* c'" := (c -[ tm ]->* c') (at level 40).
+Notation "c -->+ c'" := (c -[ tm ]->+ c') (at level 40).
+
+Notation ld := [1;1;1].
+Notation d0 := [1;0;1].
+Notation d1 := [1;0;0].
+Notation lh := (0inf<*<[1;1]).
+
+Notation hR := (A,[]).
+Notation hL := (B,[]).
+Notation h := [(hR,hL)].
+
+Inductive RD := LD|D0|D1.
+
+Fixpoint toRC ls :=
+match ls with
+| [] => [1]*>0inf
+| LD::ls => ld*>toRC ls
+| D0::ls => d0*>toRC ls
+| D1::ls => d1*>toRC ls
+end.
+
+Fixpoint toRC' ls :=
+match ls with
+| [] => 0inf
+| LD::ls => ld*>toRC' ls
+| D0::ls => [0;1;1]*>toRC' ls
+| D1::ls => [0;0;1]*>toRC' ls
+end.
+
+Lemma toRC_shift ls:
+  toRC ls = [1] *> toRC' ls.
+Proof.
+  induction ls as [|[] ls]; cbn in *; congruence.
+Qed.
+
+Lemma LRst r:
+  lh {{{ (hL,L) }}} [1] *> r -->*
+  lh {{{ (hR,R) }}} ld *> r.
+Proof.
+  er.
+Qed.
+
+
+Inductive RIncs: nat->(list RD)->(list RD)->Prop :=
+| RIncs_LD k r r':
+  RIncs (k*2) r r' ->
+  RIncs k (LD::r) (LD::r')
+| RIncs_D0 k r r':
+  RIncs (k*2) r r' ->
+  RIncs (1+k) (D0::r) (LD::r')
+| RIncs_D1_0 k r r':
+  RIncs (k) r r' ->
+  RIncs (1+k*2) (D1::r) (D0::r')
+| RIncs_D1_1 k r r':
+  RIncs (k) r r' ->
+  RIncs (2+k*2) (D1::r) (D1::r')
+| RIncs_rh_0:
+  RIncs 1 [] []
+| RIncs_rh_1 k r:
+  RIncs k [] r ->
+  RIncs (1+k*2) [] (D1::r)
+| RIncs_rh_2 k r:
+  RIncs (1+k) [] r ->
+  RIncs (2+k*2) [] (D0::r)
+.
+
+Ltac cat' :=
+  eapply segRLs_sideRLs_concat; [|eauto 1].
+
+Ltac cat'' :=
+  replace 0inf with ([0;0;0]*>0inf) by (st; reflexivity); cat'.
+
+Open Scope nat.
+
+Lemma RIncs_spec k r r':
+  RIncs k r r' ->
+  sideRLs tm (h^^k) (toRC' r) (toRC r').
+Proof.
+  intro H.
+  induction H; intros; cbn[toRC toRC'] in *.
+  - cat'. am 1 2 k 0 0.
+  - cat'. am 1 2 k 1 0.
+  - cat'. am 2 1 k 1 0.
+  - cat'. am 2 1 k 2 0.
+  - esc.
+  - cat''. am 2 1 k 1 0.
+  - cat''. am 2 1 k 2 1.
+Qed.
+
+Ltac solve_v1 H k :=
+  let I1:=fresh "I" in
+  unshelve epose proof (H k _) as [r'' I1]; [lia|repeat ec; apply I1].
+
+Ltac solve_v2 H k :=
+  let I1:=fresh "I" in
+  unshelve epose proof (H k _ _) as [r'' I1]; [lia|lia|repeat ec; apply I1].
+
+
+Lemma RIncs_nxt k r r' k':
+  RIncs k r r' ->
+  k<=k' ->
+  exists r'',
+  RIncs k' r' r''.
+Proof.
+  intro H.
+  gen k'.
+  induction H; intros.
+  - solve_v1 IHRIncs (k'*2).
+  - solve_v1 IHRIncs (k'*2).
+  - destruct (sub k' 1); [subst|lia].
+    solve_v1 IHRIncs (c*2).
+  - destruct (sub k' 1); [subst|lia].
+    destruct (mod2 c); subst.
+    + solve_v1 IHRIncs a.
+    + solve_v1 IHRIncs a.
+  - gen H.
+    induction k' using lt_wf_ind; intros.
+    destruct (sub k' 1); [subst|lia].
+    destruct (mod2 c); subst.
+    + destruct a.
+      * ec; ec.
+      * solve_v2 H (S a).
+    + solve_v2 H (1+a).
+  - destruct (sub k' 1); [subst|lia].
+    destruct (mod2 c); subst.
+    + solve_v1 IHRIncs a.
+    + solve_v1 IHRIncs a.
+  - destruct (sub k' 1); [subst|lia].
+    solve_v1 IHRIncs (c*2).
+Qed.
+
+Definition S' ls := lh {{{ (hR,R) }}} toRC' ls.
+
+Lemma RIncs' r r':
+  RIncs 1 r r' ->
+  S' r -->+
+  S' (LD::r').
+Proof.
+  unfold S'.
+  intros.
+  epose proof H as H'.
+  apply RIncs_spec in H'.
+  eapply sideRLs_1 in H'.
+  follow10 H'.
+  rewrite toRC_shift.
+  follow LRst.
+  finish.
+Qed.
+
+Lemma nonhalt: ~halts tm c0.
+Proof.
+  eapply multistep_nonhalt with (c':=S' [LD;D0]).
+  1: esx.
+  eapply progress_nonhalt_cond with (P:=fun r => exists r', RIncs 1 r r').
+  2: repeat ec.
+  intros r [r' I1].
+  epose proof I1 as I2.
+  apply RIncs' in I2.
+  ec; ec.
+  1: apply I2.
+  eapply RIncs_nxt in I1.
+  destruct I1 as [r'' I1].
+  ec. ec.
+  - apply I1.
+  - lia.
+Qed.
+
+End TM3.
+
+
+Module TM4.
+Definition tm := Eval compute in (TM_from_str "1RB1LD_1RC0LD_1RD1RE_0LA1LD_0RB0RF_---0RC").
+Notation "c -->* c'" := (c -[ tm ]->* c') (at level 40).
+Notation "c -->+ c'" := (c -[ tm ]->+ c') (at level 40).
+
+Notation ld := [1;1;1].
+Notation d0 := [1;0;1].
+Notation d1 := [1;0;0].
+Notation lh := (0inf<*<[1;1]).
+
+Notation hR := (C,[]).
+Notation hL := (D,[]).
+Notation h := [(hR,hL)].
+
+Inductive RD := LD|D0|D1.
+
+Fixpoint toRC ls :=
+match ls with
+| [] => [1]*>0inf
+| LD::ls => ld*>toRC ls
+| D0::ls => d0*>toRC ls
+| D1::ls => d1*>toRC ls
+end.
+
+Fixpoint toRC' ls :=
+match ls with
+| [] => 0inf
+| LD::ls => ld*>toRC' ls
+| D0::ls => [0;1;1]*>toRC' ls
+| D1::ls => [0;0;1]*>toRC' ls
+end.
+
+Lemma toRC_shift ls:
+  toRC ls = [1] *> toRC' ls.
+Proof.
+  induction ls as [|[] ls]; cbn in *; congruence.
+Qed.
+
+Lemma LRst r:
+  lh {{{ (hL,L) }}} [1] *> r -->*
+  lh {{{ (hR,R) }}} ld *> r.
+Proof.
+  er.
+Qed.
+
+
+Inductive RIncs: nat->(list RD)->(list RD)->Prop :=
+| RIncs_LD k r r':
+  RIncs (k*2) r r' ->
+  RIncs k (LD::r) (LD::r')
+| RIncs_D0 k r r':
+  RIncs (k*2) r r' ->
+  RIncs (1+k) (D0::r) (LD::r')
+| RIncs_D1_0 k r r':
+  RIncs (k) r r' ->
+  RIncs (1+k*2) (D1::r) (D0::r')
+| RIncs_D1_1 k r r':
+  RIncs (k) r r' ->
+  RIncs (2+k*2) (D1::r) (D1::r')
+| RIncs_rh_0:
+  RIncs 1 [] []
+| RIncs_rh_1 k r:
+  RIncs k [] r ->
+  RIncs (1+k*2) [] (D1::r)
+| RIncs_rh_2 k r:
+  RIncs (1+k) [] r ->
+  RIncs (2+k*2) [] (D0::r)
+.
+
+Ltac cat' :=
+  eapply segRLs_sideRLs_concat; [|eauto 1].
+
+Ltac cat'' :=
+  replace 0inf with ([0;0;0]*>0inf) by (st; reflexivity); cat'.
+
+Open Scope nat.
+
+Lemma RIncs_spec k r r':
+  RIncs k r r' ->
+  sideRLs tm (h^^k) (toRC' r) (toRC r').
+Proof.
+  intro H.
+  induction H; intros; cbn[toRC toRC'] in *.
+  - cat'. am 1 2 k 0 0.
+  - cat'. am 1 2 k 1 0.
+  - cat'. am 2 1 k 1 0.
+  - cat'. am 2 1 k 2 0.
+  - esc.
+  - cat''. am 2 1 k 1 0.
+  - cat''. am 2 1 k 2 1.
+Qed.
+
+Ltac solve_v1 H k :=
+  let I1:=fresh "I" in
+  unshelve epose proof (H k _) as [r'' I1]; [lia|repeat ec; apply I1].
+
+Ltac solve_v2 H k :=
+  let I1:=fresh "I" in
+  unshelve epose proof (H k _ _) as [r'' I1]; [lia|lia|repeat ec; apply I1].
+
+
+Lemma RIncs_nxt k r r' k':
+  RIncs k r r' ->
+  k<=k' ->
+  exists r'',
+  RIncs k' r' r''.
+Proof.
+  intro H.
+  gen k'.
+  induction H; intros.
+  - solve_v1 IHRIncs (k'*2).
+  - solve_v1 IHRIncs (k'*2).
+  - destruct (sub k' 1); [subst|lia].
+    solve_v1 IHRIncs (c*2).
+  - destruct (sub k' 1); [subst|lia].
+    destruct (mod2 c); subst.
+    + solve_v1 IHRIncs a.
+    + solve_v1 IHRIncs a.
+  - gen H.
+    induction k' using lt_wf_ind; intros.
+    destruct (sub k' 1); [subst|lia].
+    destruct (mod2 c); subst.
+    + destruct a.
+      * ec; ec.
+      * solve_v2 H (S a).
+    + solve_v2 H (1+a).
+  - destruct (sub k' 1); [subst|lia].
+    destruct (mod2 c); subst.
+    + solve_v1 IHRIncs a.
+    + solve_v1 IHRIncs a.
+  - destruct (sub k' 1); [subst|lia].
+    solve_v1 IHRIncs (c*2).
+Qed.
+
+Definition S' ls := lh {{{ (hR,R) }}} toRC' ls.
+
+Lemma RIncs' r r':
+  RIncs 1 r r' ->
+  S' r -->+
+  S' (LD::r').
+Proof.
+  unfold S'.
+  intros.
+  epose proof H as H'.
+  apply RIncs_spec in H'.
+  eapply sideRLs_1 in H'.
+  follow10 H'.
+  rewrite toRC_shift.
+  follow LRst.
+  finish.
+Qed.
+
+Lemma nonhalt: ~halts tm c0.
+Proof.
+  eapply multistep_nonhalt with (c':=S' [LD]).
+  1: esx.
+  eapply progress_nonhalt_cond with (P:=fun r => exists r', RIncs 1 r r').
+  2: repeat ec.
+  intros r [r' I1].
+  epose proof I1 as I2.
+  apply RIncs' in I2.
+  ec; ec.
+  1: apply I2.
+  eapply RIncs_nxt in I1.
+  destruct I1 as [r'' I1].
+  ec. ec.
+  - apply I1.
+  - lia.
+Qed.
+
+End TM4.
+
+
+Module TM5.
+Definition tm := Eval compute in (TM_from_str "1LB1RE_0LC1LB_1RD1LB_1RA0LB_0RD0RF_---0RA").
+Notation "c -->* c'" := (c -[ tm ]->* c') (at level 40).
+Notation "c -->+ c'" := (c -[ tm ]->+ c') (at level 40).
+
+Notation ld := [1;1;1].
+Notation d0 := [1;0;1].
+Notation d1 := [1;0;0].
+Notation lh := (0inf<*<[1;1]).
+
+Notation hR := (A,[]).
+Notation hL := (B,[]).
+Notation h := [(hR,hL)].
+
+Inductive RD := LD|D0|D1.
+
+Fixpoint toRC ls :=
+match ls with
+| [] => [1]*>0inf
+| LD::ls => ld*>toRC ls
+| D0::ls => d0*>toRC ls
+| D1::ls => d1*>toRC ls
+end.
+
+Fixpoint toRC' ls :=
+match ls with
+| [] => 0inf
+| LD::ls => ld*>toRC' ls
+| D0::ls => [0;1;1]*>toRC' ls
+| D1::ls => [0;0;1]*>toRC' ls
+end.
+
+Lemma toRC_shift ls:
+  toRC ls = [1] *> toRC' ls.
+Proof.
+  induction ls as [|[] ls]; cbn in *; congruence.
+Qed.
+
+Lemma LRst r:
+  lh {{{ (hL,L) }}} [1] *> r -->*
+  lh {{{ (hR,R) }}} ld *> r.
+Proof.
+  er.
+Qed.
+
+
+Inductive RIncs: nat->(list RD)->(list RD)->Prop :=
+| RIncs_LD k r r':
+  RIncs (k*2) r r' ->
+  RIncs k (LD::r) (LD::r')
+| RIncs_D0 k r r':
+  RIncs (k*2) r r' ->
+  RIncs (1+k) (D0::r) (LD::r')
+| RIncs_D1_0 k r r':
+  RIncs (k) r r' ->
+  RIncs (1+k*2) (D1::r) (D0::r')
+| RIncs_D1_1 k r r':
+  RIncs (k) r r' ->
+  RIncs (2+k*2) (D1::r) (D1::r')
+| RIncs_rh_0:
+  RIncs 1 [] []
+| RIncs_rh_1 k r:
+  RIncs k [] r ->
+  RIncs (1+k*2) [] (D1::r)
+| RIncs_rh_2 k r:
+  RIncs (1+k) [] r ->
+  RIncs (2+k*2) [] (D0::r)
+.
+
+Ltac cat' :=
+  eapply segRLs_sideRLs_concat; [|eauto 1].
+
+Ltac cat'' :=
+  replace 0inf with ([0;0;0]*>0inf) by (st; reflexivity); cat'.
+
+Open Scope nat.
+
+Lemma RIncs_spec k r r':
+  RIncs k r r' ->
+  sideRLs tm (h^^k) (toRC' r) (toRC r').
+Proof.
+  intro H.
+  induction H; intros; cbn[toRC toRC'] in *.
+  - cat'. am 1 2 k 0 0.
+  - cat'. am 1 2 k 1 0.
+  - cat'. am 2 1 k 1 0.
+  - cat'. am 2 1 k 2 0.
+  - esc.
+  - cat''. am 2 1 k 1 0.
+  - cat''. am 2 1 k 2 1.
+Qed.
+
+Ltac solve_v1 H k :=
+  let I1:=fresh "I" in
+  unshelve epose proof (H k _) as [r'' I1]; [lia|repeat ec; apply I1].
+
+Ltac solve_v2 H k :=
+  let I1:=fresh "I" in
+  unshelve epose proof (H k _ _) as [r'' I1]; [lia|lia|repeat ec; apply I1].
+
+
+Lemma RIncs_nxt k r r' k':
+  RIncs k r r' ->
+  k<=k' ->
+  exists r'',
+  RIncs k' r' r''.
+Proof.
+  intro H.
+  gen k'.
+  induction H; intros.
+  - solve_v1 IHRIncs (k'*2).
+  - solve_v1 IHRIncs (k'*2).
+  - destruct (sub k' 1); [subst|lia].
+    solve_v1 IHRIncs (c*2).
+  - destruct (sub k' 1); [subst|lia].
+    destruct (mod2 c); subst.
+    + solve_v1 IHRIncs a.
+    + solve_v1 IHRIncs a.
+  - gen H.
+    induction k' using lt_wf_ind; intros.
+    destruct (sub k' 1); [subst|lia].
+    destruct (mod2 c); subst.
+    + destruct a.
+      * ec; ec.
+      * solve_v2 H (S a).
+    + solve_v2 H (1+a).
+  - destruct (sub k' 1); [subst|lia].
+    destruct (mod2 c); subst.
+    + solve_v1 IHRIncs a.
+    + solve_v1 IHRIncs a.
+  - destruct (sub k' 1); [subst|lia].
+    solve_v1 IHRIncs (c*2).
+Qed.
+
+Definition S' ls := lh {{{ (hR,R) }}} toRC' ls.
+
+Lemma RIncs' r r':
+  RIncs 1 r r' ->
+  S' r -->+
+  S' (LD::r').
+Proof.
+  unfold S'.
+  intros.
+  epose proof H as H'.
+  apply RIncs_spec in H'.
+  eapply sideRLs_1 in H'.
+  follow10 H'.
+  rewrite toRC_shift.
+  follow LRst.
+  finish.
+Qed.
+
+Lemma nonhalt: ~halts tm c0.
+Proof.
+  eapply multistep_nonhalt with (c':=S' [LD;D0]).
+  1: esx.
+  eapply progress_nonhalt_cond with (P:=fun r => exists r', RIncs 1 r r').
+  2: repeat ec.
+  intros r [r' I1].
+  epose proof I1 as I2.
+  apply RIncs' in I2.
+  ec; ec.
+  1: apply I2.
+  eapply RIncs_nxt in I1.
+  destruct I1 as [r'' I1].
+  ec. ec.
+  - apply I1.
+  - lia.
+Qed.
+
+End TM5.
+
+
+Module TM6.
+Definition tm := Eval compute in (TM_from_str "1RB1LD_1RC0LD_1LD1RE_0LA1LD_0RB0RF_---0RC").
+Notation "c -->* c'" := (c -[ tm ]->* c') (at level 40).
+Notation "c -->+ c'" := (c -[ tm ]->+ c') (at level 40).
+
+Notation ld := [1;1;1].
+Notation d0 := [1;0;1].
+Notation d1 := [1;0;0].
+Notation lh := (0inf<*<[1;1]).
+
+Notation hR := (C,[]).
+Notation hL := (D,[]).
+Notation h := [(hR,hL)].
+
+Inductive RD := LD|D0|D1.
+
+Fixpoint toRC ls :=
+match ls with
+| [] => [1]*>0inf
+| LD::ls => ld*>toRC ls
+| D0::ls => d0*>toRC ls
+| D1::ls => d1*>toRC ls
+end.
+
+Fixpoint toRC' ls :=
+match ls with
+| [] => 0inf
+| LD::ls => ld*>toRC' ls
+| D0::ls => [0;1;1]*>toRC' ls
+| D1::ls => [0;0;1]*>toRC' ls
+end.
+
+Lemma toRC_shift ls:
+  toRC ls = [1] *> toRC' ls.
+Proof.
+  induction ls as [|[] ls]; cbn in *; congruence.
+Qed.
+
+Lemma LRst r:
+  lh {{{ (hL,L) }}} [1] *> r -->*
+  lh {{{ (hR,R) }}} ld *> r.
+Proof.
+  er.
+Qed.
+
+
+Inductive RIncs: nat->(list RD)->(list RD)->Prop :=
+| RIncs_LD k r r':
+  RIncs (k*2) r r' ->
+  RIncs k (LD::r) (LD::r')
+| RIncs_D0 k r r':
+  RIncs (k*2) r r' ->
+  RIncs (1+k) (D0::r) (LD::r')
+| RIncs_D1_0 k r r':
+  RIncs (k) r r' ->
+  RIncs (1+k*2) (D1::r) (D0::r')
+| RIncs_D1_1 k r r':
+  RIncs (k) r r' ->
+  RIncs (2+k*2) (D1::r) (D1::r')
+| RIncs_rh_0:
+  RIncs 1 [] []
+| RIncs_rh_1 k r:
+  RIncs k [] r ->
+  RIncs (1+k*2) [] (D1::r)
+| RIncs_rh_2 k r:
+  RIncs (1+k) [] r ->
+  RIncs (2+k*2) [] (D0::r)
+.
+
+Ltac cat' :=
+  eapply segRLs_sideRLs_concat; [|eauto 1].
+
+Ltac cat'' :=
+  replace 0inf with ([0;0;0]*>0inf) by (st; reflexivity); cat'.
+
+Open Scope nat.
+
+Lemma RIncs_spec k r r':
+  RIncs k r r' ->
+  sideRLs tm (h^^k) (toRC' r) (toRC r').
+Proof.
+  intro H.
+  induction H; intros; cbn[toRC toRC'] in *.
+  - cat'. am 1 2 k 0 0.
+  - cat'. am 1 2 k 1 0.
+  - cat'. am 2 1 k 1 0.
+  - cat'. am 2 1 k 2 0.
+  - esc.
+  - cat''. am 2 1 k 1 0.
+  - cat''. am 2 1 k 2 1.
+Qed.
+
+Ltac solve_v1 H k :=
+  let I1:=fresh "I" in
+  unshelve epose proof (H k _) as [r'' I1]; [lia|repeat ec; apply I1].
+
+Ltac solve_v2 H k :=
+  let I1:=fresh "I" in
+  unshelve epose proof (H k _ _) as [r'' I1]; [lia|lia|repeat ec; apply I1].
+
+
+Lemma RIncs_nxt k r r' k':
+  RIncs k r r' ->
+  k<=k' ->
+  exists r'',
+  RIncs k' r' r''.
+Proof.
+  intro H.
+  gen k'.
+  induction H; intros.
+  - solve_v1 IHRIncs (k'*2).
+  - solve_v1 IHRIncs (k'*2).
+  - destruct (sub k' 1); [subst|lia].
+    solve_v1 IHRIncs (c*2).
+  - destruct (sub k' 1); [subst|lia].
+    destruct (mod2 c); subst.
+    + solve_v1 IHRIncs a.
+    + solve_v1 IHRIncs a.
+  - gen H.
+    induction k' using lt_wf_ind; intros.
+    destruct (sub k' 1); [subst|lia].
+    destruct (mod2 c); subst.
+    + destruct a.
+      * ec; ec.
+      * solve_v2 H (S a).
+    + solve_v2 H (1+a).
+  - destruct (sub k' 1); [subst|lia].
+    destruct (mod2 c); subst.
+    + solve_v1 IHRIncs a.
+    + solve_v1 IHRIncs a.
+  - destruct (sub k' 1); [subst|lia].
+    solve_v1 IHRIncs (c*2).
+Qed.
+
+Definition S' ls := lh {{{ (hR,R) }}} toRC' ls.
+
+Lemma RIncs' r r':
+  RIncs 1 r r' ->
+  S' r -->+
+  S' (LD::r').
+Proof.
+  unfold S'.
+  intros.
+  epose proof H as H'.
+  apply RIncs_spec in H'.
+  eapply sideRLs_1 in H'.
+  follow10 H'.
+  rewrite toRC_shift.
+  follow LRst.
+  finish.
+Qed.
+
+Lemma nonhalt: ~halts tm c0.
+Proof.
+  eapply multistep_nonhalt with (c':=S' [LD]).
+  1: esx.
+  eapply progress_nonhalt_cond with (P:=fun r => exists r', RIncs 1 r r').
+  2: repeat ec.
+  intros r [r' I1].
+  epose proof I1 as I2.
+  apply RIncs' in I2.
+  ec; ec.
+  1: apply I2.
+  eapply RIncs_nxt in I1.
+  destruct I1 as [r'' I1].
+  ec. ec.
+  - apply I1.
+  - lia.
+Qed.
+
+End TM6.
+
+
+
